Resurrect pgcl example's posreal theory

examples/pgcl/src/posrealScript.sml
@@ -31,12 +31,6 @@ val _ = new_theory "posreal";
 (* Helpful proof tools                                                       *)
 (* ------------------------------------------------------------------------- *)
 
-infixr 0 ++ << || THENC ORELSEC ORELSER ##;
-infix 1 >>;
-
-val op ++ = op THEN;
-val op << = op THENL;
-val op >> = op THEN1;
 val op || = op ORELSE;
 val Know = Q_TAC KNOW_TAC;
 val Suff = Q_TAC SUFF_TAC;
@@ -53,7 +47,7 @@ val unint_def = Define `unint x = x`;
 (* ------------------------------------------------------------------------- *)
 
 val posreal_pred_def = Define
-  `(posreal_pred NONE = T) /\ (posreal_pred (SOME x) = 0r <= x)`;
+  `(posreal_pred NONE = T) /\ (posreal_pred (SOME x) <=> 0r <= x)`;
 
 val posreal_inhabited =
   prove (``?x. posreal_pred x``, METIS_TAC [posreal_pred_def]);
@@ -96,7 +90,7 @@ val preal_ler_def = Define
   `(preal_ler NONE NONE = T) /\
    (preal_ler NONE (SOME y) = F) /\
    (preal_ler (SOME x) NONE = T) /\
-   (preal_ler (SOME (x:real)) (SOME y) = x <= y)`;
+   (preal_ler (SOME (x:real)) (SOME y) <=> x <= y)`;
 
 val preal_mulr_def = Define
   `(preal_mulr NONE NONE = NONE) /\
@@ -154,11 +148,11 @@ val posreal_cases = store_thm
   ("posreal_cases",
    ``!x. (x = infty) \/ ?y. 0 <= y /\ (x = preal y)``,
    RW_TAC std_ss [preal_def, infty_def]
-   ++ MP_TAC (Q.SPEC `x` (CONJUNCT1 posreal_tybij))
-   ++ DISCH_THEN (fn th => ONCE_REWRITE_TAC [SYM th])
-   ++ Cases_on `posreal_rep x` >> RW_TAC std_ss []
-   ++ DISJ2_TAC
-   ++ METIS_TAC [posreal_pred_def, posreal_tybij, pos_def]);
+   >> MP_TAC (Q.SPEC `x` (CONJUNCT1 posreal_tybij))
+   >> DISCH_THEN (fn th => ONCE_REWRITE_TAC [SYM th])
+   >> Cases_on `posreal_rep x` >- RW_TAC std_ss []
+   >> DISJ2_TAC
+   >> METIS_TAC [posreal_pred_def, posreal_tybij, pos_def]);
 
 val posreal_trich = store_thm
   ("posreal_trich",
@@ -166,13 +160,13 @@ val posreal_trich = store_thm
        (x = 0) \/ (x = infty) \/
        ~(x = 0) /\ ?y. ~(y = 0) /\ 0 <= y /\ (x = preal y)``,
    GEN_TAC
-   ++ Cases_on `x = 0` >> RW_TAC std_ss []
-   ++ MP_TAC (Q.SPEC `x` posreal_cases)
-   ++ RW_TAC std_ss []
-   ++ DISJ2_TAC
-   ++ Q.EXISTS_TAC `y`
-   ++ RW_TAC std_ss []
-   ++ METIS_TAC [posreal_of_num_def]);
+   >> Cases_on `x = 0` >- RW_TAC std_ss []
+   >> MP_TAC (Q.SPEC `x` posreal_cases)
+   >> RW_TAC std_ss []
+   >> DISJ2_TAC
+   >> Q.EXISTS_TAC `y`
+   >> RW_TAC std_ss []
+   >> METIS_TAC [posreal_of_num_def]);
 
 local
   val posreal = Type `:posreal`;
@@ -204,40 +198,40 @@ val preal_inj = store_thm
   ("preal_inj",
    ``!x y. 0 <= x /\ 0 <= y /\ (preal x = preal y) ==> (x = y)``,
    RW_TAC std_ss [preal_def]
-   ++ Suff `pos x = pos y` >> RW_TAC real_ss [pos_def]
-   ++ ONCE_REWRITE_TAC [GSYM SOME_11]
-   ++ MATCH_MP_TAC posreal_abs_inj
-   ++ RW_TAC std_ss [posreal_pred_def, REAL_POS_POS]);
+   >> Suff `pos x = pos y` >- RW_TAC real_ss [pos_def]
+   >> ONCE_REWRITE_TAC [GSYM SOME_11]
+   >> MATCH_MP_TAC posreal_abs_inj
+   >> RW_TAC std_ss [posreal_pred_def, REAL_POS_POS]);
 
 val preal_eq_zero = store_thm
   ("preal_eq_zero",
-   ``!x. (preal x = 0) = x <= 0``,
+   ``!x. (preal x = 0) <=> x <= 0``,
    RW_TAC std_ss [preal_def, posreal_of_num_def]
-   ++ REVERSE EQ_TAC >> METIS_TAC [REAL_POS_EQ_ZERO, pos_def, REAL_LE_REFL]
-   ++ STRIP_TAC
-   ++ Know `pos x = pos 0`
-   >> METIS_TAC
+   >> REVERSE EQ_TAC >- METIS_TAC [REAL_POS_EQ_ZERO, pos_def, REAL_LE_REFL]
+   >> STRIP_TAC
+   >> Know `pos x = pos 0`
+   >- METIS_TAC
       [posreal_abs_inj, posreal_pred_def, REAL_POS_POS, optionTheory.SOME_11]
-   ++ SIMP_TAC real_ss [Q.SPEC `0` pos_def]);
+   >> SIMP_TAC real_ss [Q.SPEC `0` pos_def]);
 
 val posreal_of_num_inj = store_thm
   ("posreal_of_num_inj",
    ``!m n. (posreal_of_num m = posreal_of_num n) = (m = n)``,
    RW_TAC std_ss [posreal_of_num_def]
-   ++ REVERSE EQ_TAC >> RW_TAC std_ss []
-   ++ STRIP_TAC
-   ++ Suff `(& m : real) = & n` >> RW_TAC real_ss []
-   ++ MATCH_MP_TAC preal_inj
-   ++ RW_TAC real_ss []);
+   >> REVERSE EQ_TAC >- RW_TAC std_ss []
+   >> STRIP_TAC
+   >> Suff `(& m : real) = & n` >- RW_TAC real_ss []
+   >> MATCH_MP_TAC preal_inj
+   >> RW_TAC real_ss []);
 
 val preal_add = store_thm
   ("preal_add",
    ``!x y. 0 <= x /\ 0 <= y ==> (preal x + preal y = preal (x + y))``,
    RW_TAC std_ss [preal_add_def, preal_def, posreal_cancel, REAL_POS_POS]
-   ++ RW_TAC std_ss [preal_addr_def, pos_def]
-   ++ Suff `F` >> REWRITE_TAC []
-   ++ REPEAT (POP_ASSUM MP_TAC)
-   ++ REAL_ARITH_TAC);
+   >> RW_TAC std_ss [preal_addr_def, pos_def]
+   >> Suff `F` >- REWRITE_TAC []
+   >> REPEAT (POP_ASSUM MP_TAC)
+   >> REAL_ARITH_TAC);
 
 val posreal_of_num_add = store_thm
   ("posreal_of_num_add",
@@ -248,25 +242,25 @@ val preal_sub = store_thm
   ("preal_sub",
    ``!x y. 0 <= y ==> (preal x - preal y = preal (x - y))``,
    RW_TAC std_ss [preal_sub_def, preal_def, posreal_cancel, REAL_POS_POS]
-   ++ RW_TAC real_ss [preal_subr_def, pos_def, REAL_LE_SUB_LADD]
-   << [Suff `x = y` >> RW_TAC real_ss []
-       ++ REPEAT (POP_ASSUM MP_TAC)
-       ++ REAL_ARITH_TAC,
-       Suff `x = y` >> RW_TAC real_ss []
-       ++ REPEAT (POP_ASSUM MP_TAC)
-       ++ REAL_ARITH_TAC,
-       Suff `x = 0` >> RW_TAC real_ss []
-       ++ REPEAT (POP_ASSUM MP_TAC)
-       ++ REAL_ARITH_TAC,
-       Suff `y = 0` >> RW_TAC real_ss []
-       ++ REPEAT (POP_ASSUM MP_TAC)
-       ++ REAL_ARITH_TAC]);
+   >> RW_TAC real_ss [preal_subr_def, pos_def, REAL_LE_SUB_LADD]
+   >| [Suff `x = y` >- RW_TAC real_ss []
+       >> REPEAT (POP_ASSUM MP_TAC)
+       >> REAL_ARITH_TAC,
+       Suff `x = y` >- RW_TAC real_ss []
+       >> REPEAT (POP_ASSUM MP_TAC)
+       >> REAL_ARITH_TAC,
+       Suff `x = 0` >- RW_TAC real_ss []
+       >> REPEAT (POP_ASSUM MP_TAC)
+       >> REAL_ARITH_TAC,
+       Suff `y = 0` >- RW_TAC real_ss []
+       >> REPEAT (POP_ASSUM MP_TAC)
+       >> REAL_ARITH_TAC]);
 
 val posreal_of_num_sub = store_thm
   ("posreal_of_num_sub",
    ``!a b. posreal_of_num a - posreal_of_num b = posreal_of_num (a - b)``,
    RW_TAC std_ss [posreal_of_num_def, preal_sub, REAL_POS, REAL_SUB]
-   ++ RW_TAC std_ss
+   >> RW_TAC std_ss
       [GSYM posreal_of_num_def, preal_eq_zero, REAL_NEG_LE0, REAL_POS,
        DECIDE ``(a:num) <= b ==> (a - b = 0)``]);
 
@@ -274,8 +268,8 @@ val preal_le = store_thm
   ("preal_le",
    ``!x y. x <= y ==> preal x <= preal y``,
    RW_TAC std_ss [preal_def]
-   ++ RW_TAC std_ss [preal_le_def, posreal_cancel, preal_ler_def, REAL_POS_POS]
-   ++ METIS_TAC [REAL_POS_MONO]);
+   >> RW_TAC std_ss [preal_le_def, posreal_cancel, preal_ler_def, REAL_POS_POS]
+   >> METIS_TAC [REAL_POS_MONO]);
 
 val preal_mul = store_thm
   ("preal_mul",
@@ -283,29 +277,29 @@ val preal_mul = store_thm
    RW_TAC real_ss
    [preal_mul_def, preal_mulr_def, posreal_cancel, preal_def, REAL_POS_POS,
     pos_def]
-   << [METIS_TAC [REAL_LE_MUL],
-       Suff `x = 0` >> RW_TAC real_ss []
-       ++ Suff `~(~(x = 0) /\ 0 < x)`
-       >> (REPEAT (POP_ASSUM MP_TAC) ++ REAL_ARITH_TAC)
-       ++ STRIP_TAC
-       ++ Q.PAT_ASSUM `~(0 <= y)` MP_TAC
-       ++ Suff `~(y = 0) ==> 0 < y` >> REAL_ARITH_TAC
-       ++ STRIP_TAC
-       ++ MP_TAC (Q.SPECL [`x`, `y`] (GSYM REAL_LT_LMUL_0))
-       ++ RW_TAC std_ss [REAL_LT_LE]
-       ++ ONCE_REWRITE_TAC [EQ_SYM_EQ]
-       ++ RW_TAC std_ss [REAL_ENTIRE],
-       Suff `y = 0` >> RW_TAC real_ss []
-       ++ Suff `~(~(y = 0) /\ 0 < y)`
-       >> (REPEAT (POP_ASSUM MP_TAC) ++ REAL_ARITH_TAC)
-       ++ STRIP_TAC
-       ++ Q.PAT_ASSUM `~(0 <= x)` MP_TAC
-       ++ Suff `~(x = 0) ==> 0 < x` >> REAL_ARITH_TAC
-       ++ STRIP_TAC
-       ++ MP_TAC (Q.SPECL [`x`, `y`] (GSYM REAL_LT_RMUL_0))
-       ++ RW_TAC std_ss [REAL_LT_LE]
-       ++ ONCE_REWRITE_TAC [EQ_SYM_EQ]
-       ++ RW_TAC std_ss [REAL_ENTIRE]]);
+   >| [METIS_TAC [REAL_LE_MUL],
+       Suff `x = 0` >- RW_TAC real_ss []
+       >> Suff `~(~(x = 0) /\ 0 < x)`
+       >- (REPEAT (POP_ASSUM MP_TAC) >> REAL_ARITH_TAC)
+       >> STRIP_TAC
+       >> Q.PAT_X_ASSUM `~(0 <= y)` MP_TAC
+       >> Suff `~(y = 0) ==> 0 < y` >- REAL_ARITH_TAC
+       >> STRIP_TAC
+       >> MP_TAC (Q.SPECL [`x`, `y`] (GSYM REAL_LT_LMUL_0))
+       >> RW_TAC std_ss [REAL_LT_LE]
+       >> ONCE_REWRITE_TAC [EQ_SYM_EQ]
+       >> RW_TAC std_ss [REAL_ENTIRE],
+       Suff `y = 0` >- RW_TAC real_ss []
+       >> Suff `~(~(y = 0) /\ 0 < y)`
+       >- (REPEAT (POP_ASSUM MP_TAC) >> REAL_ARITH_TAC)
+       >> STRIP_TAC
+       >> Q.PAT_X_ASSUM `~(0 <= x)` MP_TAC
+       >> Suff `~(x = 0) ==> 0 < x` >- REAL_ARITH_TAC
+       >> STRIP_TAC
+       >> MP_TAC (Q.SPECL [`x`, `y`] (GSYM REAL_LT_RMUL_0))
+       >> RW_TAC std_ss [REAL_LT_LE]
+       >> ONCE_REWRITE_TAC [EQ_SYM_EQ]
+       >> RW_TAC std_ss [REAL_ENTIRE]]);
 
 val posreal_of_num_mul = store_thm
   ("posreal_of_num_mul",
@@ -316,17 +310,17 @@ val le_preal = store_thm
   ("le_preal",
    ``!x y. 0 <= y /\ preal x <= preal y ==> x <= y``,
    RW_TAC std_ss [preal_def]
-   ++ POP_ASSUM MP_TAC
-   ++ RW_TAC std_ss
+   >> POP_ASSUM MP_TAC
+   >> RW_TAC std_ss
       [preal_le_def, posreal_cancel, preal_ler_def, REAL_POS_POS, pos_def]
-   ++ REPEAT (POP_ASSUM MP_TAC)
-   ++ REAL_ARITH_TAC);
+   >> REPEAT (POP_ASSUM MP_TAC)
+   >> REAL_ARITH_TAC);
 
 val preal_not_infty = store_thm
   ("preal_not_infty",
    ``!x. ~(preal x = infty)``,
    RW_TAC std_ss [preal_def, infty_def]
-   ++ METIS_TAC [REAL_POS_POS, posreal_pred_def, posreal_tybij, NOT_SOME_NONE]);
+   >> METIS_TAC [REAL_POS_POS, posreal_pred_def, posreal_tybij, NOT_SOME_NONE]);
 
 val posreal_of_num_not_infty = store_thm
   ("posreal_of_num_not_infty",
@@ -337,90 +331,90 @@ val le_refl = store_thm
   ("le_refl",
    ``!x. x <= x``,
    pcases
-   ++ RW_TAC real_ss
+   >> RW_TAC real_ss
       [infty_def, preal_def, preal_le_def, posreal_cancel, preal_ler_def]);
 
 val le_infty = store_thm
   ("le_infty",
    ``!x. x <= infty``,
    pcases
-   ++ RW_TAC real_ss
+   >> RW_TAC real_ss
       [infty_def, preal_le_def, preal_def, posreal_cancel, preal_ler_def]);
 
 val infty_le = store_thm
   ("infty_le",
-   ``!x. infty <= x = (x = infty)``,
+   ``!x. infty <= x <=> (x = infty)``,
    pcases
-   ++ RW_TAC real_ss [le_refl, preal_not_infty]
-   ++ RW_TAC real_ss
+   >> RW_TAC real_ss [le_refl, preal_not_infty]
+   >> RW_TAC real_ss
       [infty_def, preal_le_def, preal_def, posreal_cancel, preal_ler_def]);
 
 val zero_le = store_thm
   ("zero_le",
    ``!x. 0 <= x``,
    pcases
-   ++ RW_TAC real_ss
+   >> RW_TAC real_ss
       [preal_le_def, preal_def, posreal_of_num_def, posreal_cancel, infty_def,
        preal_ler_def, REAL_POS_POS]
-   ++ METIS_TAC [REAL_POS_MONO]);
+   >> METIS_TAC [REAL_POS_MONO]);
 
 val le_zero = store_thm
   ("le_zero",
-   ``!x. x <= 0 = (x = 0)``,
-   pcases >> (RW_TAC real_ss [infty_le] ++ PROVE_TAC [])
-   ++ RW_TAC real_ss
+   ``!x. x <= 0 <=> (x = 0)``,
+   pcases >- (RW_TAC real_ss [infty_le] >> PROVE_TAC [])
+   >> RW_TAC real_ss
       [preal_le_def, preal_def, posreal_of_num_def, posreal_cancel,
        preal_ler_def, REAL_POS_POS]
-   ++ RW_TAC std_ss [pos_def]
-   ++ Know `y <= 0 = (y = 0)` >> (POP_ASSUM MP_TAC ++ REAL_ARITH_TAC)
-   ++ DISCH_THEN (fn th => REWRITE_TAC [th])
-   ++ EQ_TAC >> RW_TAC std_ss []
-   ++ METIS_TAC [posreal_abs_inj, posreal_pred_def, REAL_LE_REFL, SOME_11]);
+   >> RW_TAC std_ss [pos_def]
+   >> Know `y <= 0 <=> (y = 0)` >- (POP_ASSUM MP_TAC >> REAL_ARITH_TAC)
+   >> DISCH_THEN (fn th => REWRITE_TAC [th])
+   >> EQ_TAC >- RW_TAC std_ss []
+   >> METIS_TAC [posreal_abs_inj, posreal_pred_def, REAL_LE_REFL, SOME_11]);
 
 val le_antisym = store_thm
   ("le_antisym",
    ``!x y. x <= y /\ y <= x ==> (x = y)``,
    pcases
-   ++ pcases
-   ++ RW_TAC std_ss [infty_le, le_infty, preal_not_infty]
-   ++ PROVE_TAC [le_preal, REAL_LE_ANTISYM]);
+   >> pcases
+   >> RW_TAC std_ss [infty_le, le_infty, preal_not_infty]
+   >> PROVE_TAC [le_preal, REAL_LE_ANTISYM]);
 
 val le_trans = store_thm
   ("le_trans",
    ``!x y z. x <= y /\ y <= z ==> x <= z``,
    REPEAT pcases
-   ++ RW_TAC real_ss [infty_le, le_refl, le_infty]
-   ++ METIS_TAC [preal_le, le_preal, REAL_LE_TRANS, infty_le, preal_not_infty]);
+   >> RW_TAC real_ss [infty_le, le_refl, le_infty]
+   >> METIS_TAC [preal_le, le_preal, REAL_LE_TRANS, infty_le, preal_not_infty]);
 
 val le_total = store_thm
   ("le_total",
    ``!x y. x <= y \/ y <= x``,
-   (REPEAT pcases ++ RW_TAC std_ss [le_infty, infty_le])
-   ++ PROVE_TAC [le_preal, preal_le, REAL_LE_TOTAL]);
+   (REPEAT pcases >> RW_TAC std_ss [le_infty, infty_le])
+   >> PROVE_TAC [le_preal, preal_le, REAL_LE_TOTAL]);
 
 val add_comm = store_thm
   ("add_comm",
    ``!x y. x + y = y + x``,
    REPEAT pcases
-   ++ RW_TAC std_ss
+   >> RW_TAC std_ss
       [preal_add_def, preal_addr_def, posreal_cancel, infty_def,
        preal_def, REAL_POS_POS]
-   ++ METIS_TAC [REAL_ADD_SYM]);
+   >> METIS_TAC [REAL_ADD_SYM]);
 
 val add_assoc = store_thm
   ("add_assoc",
    ``!x y z. x + y + z = x + (y + z)``,
    REPEAT pcases
-   ++ RW_TAC real_ss
+   >> RW_TAC real_ss
       [infty_def, preal_def, posreal_cancel, preal_add_def, preal_addr_def,
        REAL_LE_ADD]
-   ++ METIS_TAC [REAL_ADD_ASSOC]);
+   >> METIS_TAC [REAL_ADD_ASSOC]);
 
 val infty_ladd = store_thm
   ("infty_ladd",
    ``!x. infty + x = infty``,
    pcases
-   ++ RW_TAC std_ss
+   >> RW_TAC std_ss
       [preal_add_def, preal_addr_def, posreal_cancel, infty_def,
        preal_def, REAL_POS_POS]);
 
@@ -433,53 +427,53 @@ val le_add2 = store_thm
   ("le_add2",
    ``!x1 x2 y1 y2. x1 <= y1 /\ x2 <= y2 ==> x1 + x2 <= y1 + y2``,
    REPEAT pcases
-   ++ RW_TAC std_ss
+   >> RW_TAC std_ss
       [preal_add, infty_ladd, infty_radd, infty_le, le_infty, preal_not_infty]
-   ++ METIS_TAC [preal_le, le_preal, REAL_LE_ADD2]);
+   >> METIS_TAC [preal_le, le_preal, REAL_LE_ADD2]);
 
 val sub_sub2 = store_thm
   ("sub_sub2",
    ``!x y. y <= x /\ ~(x = infty) ==> (x - (x - y) = y)``,
    pcases
-   ++ pcases >> RW_TAC std_ss [infty_le, preal_not_infty]
-   ++ RW_TAC std_ss [preal_not_infty]
-   ++ Know `y' <= y` >> METIS_TAC [le_preal]
-   ++ POP_ASSUM (K ALL_TAC)
-   ++ RW_TAC std_ss [preal_sub]
-   ++ Suff `0 <= y - y' /\ y - y' <= y` >> RW_TAC real_ss [preal_sub]
-   ++ REPEAT (POP_ASSUM MP_TAC)
-   ++ REAL_ARITH_TAC);
+   >> pcases >- RW_TAC std_ss [infty_le, preal_not_infty]
+   >> RW_TAC std_ss [preal_not_infty]
+   >> Know `y' <= y` >- METIS_TAC [le_preal]
+   >> POP_ASSUM (K ALL_TAC)
+   >> RW_TAC std_ss [preal_sub]
+   >> Suff `0 <= y - y' /\ y - y' <= y` >- RW_TAC real_ss [preal_sub]
+   >> REPEAT (POP_ASSUM MP_TAC)
+   >> REAL_ARITH_TAC);
 
 val le_sub_ladd = store_thm
   ("le_sub_ladd",
-   ``!x y z. z <= y /\ ~(y = infty) ==> (x <= y - z = x + z <= y)``,
-   (REPEAT pcases ++ RW_TAC std_ss [le_infty, infty_le, infty_ladd])
-   >> METIS_TAC [preal_not_infty, le_preal, preal_sub]
-   ++ Know `y'' <= y'` >> METIS_TAC [le_preal]
-   ++ RW_TAC std_ss [preal_sub, preal_add]
-   ++ Suff `0 <= y' - y''` >> METIS_TAC [preal_le, le_preal, REAL_LE_SUB_LADD]
-   ++ POP_ASSUM MP_TAC
-   ++ REAL_ARITH_TAC);
+   ``!x y z. z <= y /\ y ≠ infty ==> (x <= y - z <=> x + z <= y)``,
+   (REPEAT pcases >> RW_TAC std_ss [le_infty, infty_le, infty_ladd])
+   >- METIS_TAC [preal_not_infty, le_preal, preal_sub]
+   >> Know `y'' <= y'` >- METIS_TAC [le_preal]
+   >> RW_TAC std_ss [preal_sub, preal_add]
+   >> Suff `0 <= y' - y''` >- METIS_TAC [preal_le, le_preal, REAL_LE_SUB_LADD]
+   >> POP_ASSUM MP_TAC
+   >> REAL_ARITH_TAC);
 
 val sub_decrease = store_thm
   ("sub_decrease",
    ``!x y. ~(x = infty) \/ ~(y = infty) ==> (x - y <= x)``,
-   (REPEAT pcases ++ RW_TAC std_ss [le_infty, infty_le, preal_not_infty])
-   ++ RW_TAC real_ss
+   (REPEAT pcases >> RW_TAC std_ss [le_infty, infty_le, preal_not_infty])
+   >> RW_TAC real_ss
       [preal_le_def, preal_def, preal_ler_def, posreal_cancel, REAL_POS_POS,
        infty_def, preal_sub_def, preal_subr_def]
-   ++ POP_ASSUM MP_TAC
-   ++ RW_TAC std_ss [pos_def]
-   ++ Know `0 <= y - y'` >> (REPEAT (POP_ASSUM MP_TAC) ++ REAL_ARITH_TAC)
-   ++ RW_TAC std_ss [posreal_cancel, preal_ler_def]
-   ++ REPEAT (POP_ASSUM MP_TAC)
-   ++ REAL_ARITH_TAC);
+   >> POP_ASSUM MP_TAC
+   >> RW_TAC std_ss [pos_def]
+   >> Know `0 <= y - y'` >- (REPEAT (POP_ASSUM MP_TAC) >> REAL_ARITH_TAC)
+   >> RW_TAC std_ss [posreal_cancel, preal_ler_def]
+   >> REPEAT (POP_ASSUM MP_TAC)
+   >> REAL_ARITH_TAC);
 
 val sub_linfty = store_thm
   ("sub_linfty",
    ``!x. ~(x = infty) ==> (infty - x = infty)``,
    pcases
-   ++ RW_TAC std_ss
+   >> RW_TAC std_ss
       [preal_sub_def, infty_def, preal_def, posreal_cancel, preal_subr_def,
        REAL_POS_POS]);
 
@@ -487,7 +481,7 @@ val sub_rinfty = store_thm
   ("sub_rinfty",
    ``!x. ~(x = infty) ==> (x - infty = 0)``,
    pcases
-   ++ RW_TAC std_ss
+   >> RW_TAC std_ss
       [preal_sub_def, infty_def, preal_def, posreal_cancel, preal_subr_def,
        REAL_POS_POS, posreal_of_num_def, pos_def]);
 
@@ -495,61 +489,61 @@ val sub_mono = store_thm
   ("sub_mono",
    ``!x y z. ~(z = infty) /\ x <= y ==> x - z <= y - z``,
    REPEAT pcases
-   ++ RW_TAC std_ss [preal_sub, sub_linfty, infty_le, preal_not_infty, le_infty]
-   ++ MATCH_MP_TAC preal_le
-   ++ RW_TAC real_ss []
-   ++ METIS_TAC [le_preal]);
+   >> RW_TAC std_ss [preal_sub, sub_linfty, infty_le, preal_not_infty, le_infty]
+   >> MATCH_MP_TAC preal_le
+   >> RW_TAC real_ss []
+   >> METIS_TAC [le_preal]);
 
 val le_epsilon = store_thm
   ("le_epsilon",
    ``!x y. (!e. ~(e = 0) ==> x <= y + e) ==> x <= y``,
-   (REPEAT pcases ++ RW_TAC std_ss [le_infty, infty_le])
-   >> (POP_ASSUM MP_TAC
-       ++ RW_TAC std_ss [preal_not_infty]
-       ++ Q.EXISTS_TAC `1`
-       ++ CONJ_TAC >> RW_TAC arith_ss [posreal_of_num_inj]
-       ++ RW_TAC real_ss [posreal_of_num_def, preal_add, preal_not_infty])
-   ++ MATCH_MP_TAC preal_le
-   ++ MATCH_MP_TAC REAL_LE_EPSILON
-   ++ RW_TAC std_ss [REAL_LT_LE]
-   ++ Q.PAT_ASSUM `!e. P e` (MP_TAC o Q.SPEC `preal e`)
-   ++ MATCH_MP_TAC (PROVE [] ``x /\ (y ==> z) ==> (x ==> y) ==> z``)
-   ++ CONJ_TAC
-   >> (RW_TAC std_ss [posreal_of_num_def]
-       ++ METIS_TAC [preal_inj, REAL_LE_REFL])
-   ++ RW_TAC std_ss [preal_add]
-   ++ METIS_TAC [le_preal, REAL_LE_ADD]);
+   (REPEAT pcases >> RW_TAC std_ss [le_infty, infty_le])
+   >- (POP_ASSUM MP_TAC
+       >> RW_TAC std_ss [preal_not_infty]
+       >> Q.EXISTS_TAC `1`
+       >> CONJ_TAC >- RW_TAC arith_ss [posreal_of_num_inj]
+       >> RW_TAC real_ss [posreal_of_num_def, preal_add, preal_not_infty])
+   >> MATCH_MP_TAC preal_le
+   >> MATCH_MP_TAC REAL_LE_EPSILON
+   >> RW_TAC std_ss [REAL_LT_LE]
+   >> Q.PAT_X_ASSUM `!e. P e` (MP_TAC o Q.SPEC `preal e`)
+   >> MATCH_MP_TAC (PROVE [] ``x /\ (y ==> z) ==> (x ==> y) ==> z``)
+   >> CONJ_TAC
+   >- (RW_TAC std_ss [posreal_of_num_def]
+       >> METIS_TAC [preal_inj, REAL_LE_REFL])
+   >> RW_TAC std_ss [preal_add]
+   >> METIS_TAC [le_preal, REAL_LE_ADD]);
 
 val let_trans = store_thm
   ("let_trans",
    ``!x y z. x <= y /\ y < z ==> x < z``,
    RW_TAC std_ss [preal_lt_def]
-   ++ METIS_TAC [le_trans, le_total]);
+   >> METIS_TAC [le_trans, le_total]);
 
 val lte_trans = store_thm
   ("lte_trans",
    ``!x y z. x < y /\ y <= z ==> x < z``,
    RW_TAC std_ss [preal_lt_def]
-   ++ METIS_TAC [le_trans, le_total]);
+   >> METIS_TAC [le_trans, le_total]);
 
 val lt_le = store_thm
   ("lt_le",
    ``!x y. x < y ==> x <= y``,
    RW_TAC std_ss [preal_lt_def]
-   ++ METIS_TAC [le_total]);
+   >> METIS_TAC [le_total]);
 
 val posreal_of_num_le = store_thm
   ("posreal_of_num_le",
-   ``!m n. posreal_of_num m <= posreal_of_num n = m <= n``,
+   ``!m n. posreal_of_num m <= posreal_of_num n <=> m <= n``,
    RW_TAC std_ss [posreal_of_num_def]
-   ++ MATCH_MP_TAC EQ_TRANS
-   ++ Q.EXISTS_TAC `real_of_num m <= real_of_num n`
-   ++ REVERSE CONJ_TAC >> RW_TAC real_ss []
-   ++ METIS_TAC [le_preal, preal_le, REAL_POS]);
+   >> MATCH_MP_TAC EQ_TRANS
+   >> Q.EXISTS_TAC `real_of_num m <= real_of_num n`
+   >> REVERSE CONJ_TAC >- RW_TAC real_ss []
+   >> METIS_TAC [le_preal, preal_le, REAL_POS]);
 
 val posreal_of_num_lt = store_thm
   ("posreal_of_num_lt",
-   ``!m n. posreal_of_num m < posreal_of_num n = m < n``,
+   ``!m n. posreal_of_num m < posreal_of_num n <=> m < n``,
    METIS_TAC
    [posreal_of_num_le, preal_lt_def, arithmeticTheory.NOT_LESS_EQUAL]);
 
@@ -557,7 +551,7 @@ val add_rinfty = store_thm
   ("add_rinfty",
    ``!x. x + infty = infty``,
    pcases
-   ++ RW_TAC std_ss
+   >> RW_TAC std_ss
       [posreal_cancel, preal_add_def, preal_addr_def, REAL_POS_POS,
        infty_def, preal_def]);
 
@@ -570,10 +564,10 @@ val add_rzero = store_thm
   ("add_rzero",
    ``!x. x + 0 = x``,
    pcases
-   ++ RW_TAC std_ss
+   >> RW_TAC std_ss
       [posreal_cancel, preal_add_def, preal_addr_def, REAL_POS_POS,
        infty_def, preal_def, posreal_of_num_def]
-   ++ RW_TAC real_ss [pos_def]);
+   >> RW_TAC real_ss [pos_def]);
 
 val add_lzero = store_thm
   ("add_lzero",
@@ -582,40 +576,40 @@ val add_lzero = store_thm
 
 val le_ladd = store_thm
   ("le_ladd",
-   ``!x y z. x + y <= x + z = (x = infty) \/ y <= z``,
+   ``!x y z. x + y <= x + z <=> x = infty \/ y <= z``,
    RW_TAC std_ss []
-   ++ REVERSE EQ_TAC >> METIS_TAC [le_add2, le_refl, add_linfty]
-   ++ pcases_on `x`
-   ++ SIMP_TAC std_ss [preal_not_infty]
-   ++ pcases_on `z` >> RW_TAC std_ss [le_infty]
-   ++ pcases_on `y`
-   >> RW_TAC std_ss [add_rinfty, infty_le, preal_add, preal_not_infty]
-   ++ RW_TAC std_ss [preal_add]
-   ++ METIS_TAC [preal_le, le_preal, REAL_LE_ADD, REAL_LE_LADD]);
+   >> REVERSE EQ_TAC >- METIS_TAC [le_add2, le_refl, add_linfty]
+   >> pcases_on `x`
+   >> SIMP_TAC std_ss [preal_not_infty]
+   >> pcases_on `z` >- RW_TAC std_ss [le_infty]
+   >> pcases_on `y`
+   >- RW_TAC std_ss [add_rinfty, infty_le, preal_add, preal_not_infty]
+   >> RW_TAC std_ss [preal_add]
+   >> METIS_TAC [preal_le, le_preal, REAL_LE_ADD, REAL_LE_LADD]);
 
 val le_radd = store_thm
   ("le_radd",
-   ``!x y z. y + x <= z + x = (x = infty) \/ y <= z``,
+   ``!x y z. y + x <= z + x <=> x = infty \/ y <= z``,
    METIS_TAC [le_ladd, add_comm]);
 
 val addl_le = store_thm
   ("addl_le",
-   ``!x y. x + y <= y = (x = 0) \/ (y = infty)``,
+   ``!x y. x + y <= y <=> x = 0 \/ (y = infty)``,
    RW_TAC std_ss []
-   ++ MP_TAC (Q.SPECL [`y`, `x`, `0`] le_radd)
-   ++ METIS_TAC [le_zero, add_lzero]);
+   >> MP_TAC (Q.SPECL [`y`, `x`, `0`] le_radd)
+   >> METIS_TAC [le_zero, add_lzero]);
 
 val addr_le = store_thm
   ("addr_le",
-   ``!x y. y + x <= y = (x = 0) \/ (y = infty)``,
+   ``!x y. y + x <= y <=> x = 0 \/ y = infty``,
    METIS_TAC [addl_le, add_comm]);
 
 val le_addl = store_thm
   ("le_addl",
    ``!x y. y <= x + y``,
    RW_TAC std_ss []
-   ++ MP_TAC (Q.SPECL [`y`, `0`, `x`] le_radd)
-   ++ RW_TAC std_ss [add_lzero, zero_le]);
+   >> MP_TAC (Q.SPECL [`y`, `0`, `x`] le_radd)
+   >> RW_TAC std_ss [add_lzero, zero_le]);
 
 val le_addr = store_thm
   ("le_addr",
@@ -624,12 +618,12 @@ val le_addr = store_thm
 
 val lt_addr = store_thm
   ("lt_addr",
-   ``!x y. y < y + x = ~(x = 0) /\ ~(y = infty)``,
+   ``!x y. y < y + x <=> x ≠ 0 /\ y ≠ infty``,
    METIS_TAC [addr_le, preal_lt_def]);
 
 val lt_addl = store_thm
   ("lt_addl",
-   ``!x y. y < x + y = ~(x = 0) /\ ~(y = infty)``,
+   ``!x y. y < x + y <=> ~(x = 0) /\ ~(y = infty)``,
    METIS_TAC [lt_addr, add_comm]);
 
 val addr_lt = store_thm
@@ -646,107 +640,108 @@ val sub_le_imp = store_thm
   ("sub_le_imp",
    ``!x y z. (~(x = infty) \/ ~(y = infty)) /\ y <= z + x ==> y - x <= z``,
    REPEAT pcases
-   ++ RW_TAC std_ss
+   >> RW_TAC std_ss
       [le_infty, infty_le, sub_linfty, sub_rinfty, zero_le, preal_not_infty,
        preal_add, preal_sub]
-   ++ METIS_TAC [preal_le, le_preal, REAL_LE_SUB_RADD, REAL_LE_ADD]);
+   >> METIS_TAC [preal_le, le_preal, REAL_LE_SUB_RADD, REAL_LE_ADD]);
 
 val le_sub_imp = store_thm
   ("le_sub_imp",
    ``!x y z. (~(x = infty) \/ ~(z = infty)) /\ y + x <= z ==> y <= z - x``,
    REPEAT pcases
-   ++ RW_TAC std_ss
+   >> RW_TAC std_ss
       [le_infty, infty_le, sub_linfty, sub_rinfty, zero_le, preal_not_infty,
        preal_add, preal_sub, le_zero, add_linfty, add_rinfty]
-   ++ METIS_TAC [preal_le, le_preal, REAL_LE_SUB_LADD, REAL_LE_ADD]);
+   >> METIS_TAC [preal_le, le_preal, REAL_LE_SUB_LADD, REAL_LE_ADD]);
 
 val lt_sub_imp = store_thm
   ("lt_sub_imp",
    ``!x y z. (~(x = infty) \/ ~(z = infty)) /\ y + x < z ==> y < z - x``,
    REPEAT pcases
-   ++ RW_TAC std_ss
+   >> RW_TAC std_ss
       [le_infty, infty_le, sub_linfty, sub_rinfty, zero_le, preal_not_infty,
        preal_add, preal_sub, preal_lt_def, add_rinfty, add_linfty]
-   ++ METIS_TAC [preal_le, le_preal, REAL_LE_SUB_RADD, REAL_LE_ADD]);
+   >> METIS_TAC [preal_le, le_preal, REAL_LE_SUB_RADD, REAL_LE_ADD]);
 
 val sub_lt_imp = store_thm
   ("sub_lt_imp",
    ``!x y z.
-       (~(z = 0) /\ (~(x = infty) \/ ~(y = infty))) /\ y < z + x ==>
+       z ≠ 0 /\ (x ≠ infty \/ y ≠ infty) /\ y < z + x ==>
        y - x < z``,
    (REPEAT pcases
-    ++ RW_TAC std_ss
+    >> RW_TAC std_ss
        [le_infty, infty_le, sub_linfty, sub_rinfty, zero_le, preal_not_infty,
         preal_add, preal_sub, le_zero, add_linfty, add_rinfty, preal_lt_def,
         posreal_of_num_def])
-   >> (STRIP_TAC
-       ++ Q.PAT_ASSUM `~X` MP_TAC
-       ++ Suff `y' = 0` >> RW_TAC std_ss []
-       ++ ASM_REWRITE_TAC [GSYM REAL_LE_ANTISYM]
-       ++ METIS_TAC [le_preal, REAL_LE_REFL])
-   ++ STRIP_TAC
-   ++ Q.PAT_ASSUM `~X` MP_TAC
-   ++ REWRITE_TAC []
-   ++ MATCH_MP_TAC preal_le
-   ++ RW_TAC std_ss [GSYM REAL_LE_SUB_LADD]
-   ++ Suff `0 <= y' - y` >> METIS_TAC [le_preal]
-   ++ CCONTR_TAC
-   ++ Q.PAT_ASSUM `~(X = Y)` MP_TAC
-   ++ REWRITE_TAC []
-   ++ MATCH_MP_TAC le_antisym
-   ++ REVERSE CONJ_TAC >> RW_TAC std_ss [GSYM posreal_of_num_def, zero_le]
-   ++ Q.PAT_ASSUM `X <= Y` MP_TAC
-   ++ RW_TAC std_ss [preal_def, pos_def]);
+   >- (STRIP_TAC
+       >> Q.PAT_X_ASSUM `~X` MP_TAC
+       >> Suff `y' = 0` >- RW_TAC std_ss []
+       >> ASM_REWRITE_TAC [GSYM REAL_LE_ANTISYM]
+       >> METIS_TAC [le_preal, REAL_LE_REFL])
+   >> STRIP_TAC
+   >> Q.PAT_X_ASSUM `~X` MP_TAC
+   >> REWRITE_TAC []
+   >> MATCH_MP_TAC preal_le
+   >> RW_TAC std_ss [GSYM REAL_LE_SUB_LADD]
+   >> Suff `0 <= y' - y` >- METIS_TAC [le_preal]
+   >> CCONTR_TAC
+   >> Q.PAT_X_ASSUM `~(X = Y)` MP_TAC
+   >> REWRITE_TAC []
+   >> MATCH_MP_TAC le_antisym
+   >> REVERSE CONJ_TAC >- RW_TAC std_ss [GSYM posreal_of_num_def, zero_le]
+   >> Q.PAT_X_ASSUM `X <= Y` MP_TAC
+   >> RW_TAC std_ss [preal_def, pos_def]);
 
-val preal_le_eq = store_thm
-  ("preal_le_eq",
-   ``!x y. 0 <= x /\ 0 <= y ==> (preal x <= preal y = x <= y)``,
-   METIS_TAC [preal_le, le_preal]);
+Theorem preal_le_eq0:
+   !x y. 0 <= x /\ 0 <= y ==> (preal x <= preal y <=> x <= y)
+Proof
+  METIS_TAC [preal_le, le_preal]
+QED
 
 val preal_lt_eq = store_thm
   ("preal_lt_eq",
-   ``!x y. 0 <= x /\ 0 <= y ==> (preal x < preal y = x < y)``,
-   METIS_TAC [preal_lt_def, real_lt, preal_le_eq]);
+   ``!x y. 0 <= x /\ 0 <= y ==> (preal x < preal y <=> x < y)``,
+   METIS_TAC [preal_lt_def, real_lt, preal_le_eq0]);
 
 val sub_lzero = store_thm
   ("sub_lzero",
    ``!x. 0 - x = 0``,
    pcases
-   ++ RW_TAC real_ss
+   >> RW_TAC real_ss
       [posreal_of_num_def, preal_def, infty_def, preal_sub_def,
        posreal_cancel, REAL_POS_POS, preal_subr_def]
-   ++ FULL_SIMP_TAC real_ss [pos_def]
-   ++ PROVE_TAC []);
+   >> FULL_SIMP_TAC real_ss [pos_def]
+   >> PROVE_TAC []);
 
 val sub_rzero = store_thm
   ("sub_rzero",
    ``!x. x - 0 = x``,
    pcases
-   ++ RW_TAC real_ss
+   >> RW_TAC real_ss
       [posreal_of_num_def, preal_def, infty_def, preal_sub_def,
        posreal_cancel, REAL_POS_POS, preal_subr_def]
-   ++ FULL_SIMP_TAC real_ss [pos_def]
-   ++ PROVE_TAC [REAL_LE_ANTISYM]);
+   >> FULL_SIMP_TAC real_ss [pos_def]
+   >> PROVE_TAC [REAL_LE_ANTISYM]);
 
 val le_imp_sub_zero = store_thm
   ("le_imp_sub_zero",
    ``!x y. (~(x = infty) \/ ~(y = infty)) /\ x <= y ==> (x - y = 0)``,
    RW_TAC real_ss [GSYM le_zero]
-   ++ MATCH_MP_TAC sub_le_imp
-   ++ METIS_TAC [add_lzero]);
+   >> MATCH_MP_TAC sub_le_imp
+   >> METIS_TAC [add_lzero]);
 
 val sub_zero_imp_le = store_thm
   ("sub_zero_imp_le",
    ``!x y. (~(x = infty) \/ ~(y = infty)) /\ (x - y = 0) ==> x <= y``,
    REPEAT pcases
-   ++ RW_TAC real_ss
+   >> RW_TAC real_ss
       [le_infty, infty_le, sub_linfty, preal_not_infty,
        posreal_of_num_not_infty, preal_sub]
-   ++ MATCH_MP_TAC preal_le
-   ++ Suff `y - y' <= 0` >> REAL_ARITH_TAC
-   ++ Suff `pos (y - y') = 0` >> RW_TAC real_ss []
-   ++ FULL_SIMP_TAC std_ss [preal_def, posreal_of_num_def]
-   ++ METIS_TAC
+   >> MATCH_MP_TAC preal_le
+   >> Suff `y - y' <= 0` >- REAL_ARITH_TAC
+   >> Suff `pos (y - y') = 0` >- RW_TAC real_ss []
+   >> FULL_SIMP_TAC std_ss [preal_def, posreal_of_num_def]
+   >> METIS_TAC
       [posreal_abs_inj, posreal_pred_def, REAL_POS_POS, pos_def, REAL_LE_REFL,
        optionTheory.SOME_11]);
 
@@ -754,90 +749,92 @@ val sub_add2 = store_thm
   ("sub_add2",
    ``!x y. x <= y /\ ~(x = infty) ==> (x + (y - x) = y)``,
    REPEAT pcases
-   ++ RW_TAC real_ss
+   >> RW_TAC real_ss
       [le_infty, infty_le, sub_linfty, preal_not_infty,
        posreal_of_num_not_infty, preal_sub, add_rinfty]
-   ++ Know `0 <= y' - y`
-   >> (Suff `y <= y'` >> REAL_ARITH_TAC ++ METIS_TAC [le_preal])
-   ++ STRIP_TAC
-   ++ RW_TAC real_ss [preal_add]);
+   >> Know `0 <= y' - y`
+   >- (Suff `y <= y'` >- REAL_ARITH_TAC >> METIS_TAC [le_preal])
+   >> STRIP_TAC
+   >> RW_TAC real_ss [preal_add]);
 
-val preal_add_eq = store_thm
-  ("preal_add_eq",
-   ``!x y.
-       preal x + preal y =
-       if 0 <= x then if 0 <= y then preal (x + y) else preal x else preal y``,
+Theorem preal_add_eq:
+  !x y.
+    preal x + preal y =
+    if 0 <= x then if 0 <= y then preal (x + y) else preal x else preal y
+Proof
    RW_TAC real_ss [preal_add]
-   ++ RW_TAC real_ss [preal_def, pos_def]
-   ++ Know `0r <= 0` >> RW_TAC real_ss []
-   ++ STRIP_TAC
-   ++ IMP_RES_TAC (GSYM REAL_POS_ID)
-   ++ ASSUM_LIST ONCE_REWRITE_TAC
-   ++ SIMP_TAC std_ss
-      [GSYM preal_def, GSYM posreal_of_num_def, add_rzero, add_lzero]);
+   >> RW_TAC real_ss [preal_def, pos_def]
+   >> (Know `0r <= 0` >- RW_TAC real_ss [])
+   >> STRIP_TAC
+   >> IMP_RES_TAC (GSYM REAL_POS_ID)
+   >> ASSUM_LIST ONCE_REWRITE_TAC
+   >> SIMP_TAC std_ss
+      [GSYM preal_def, GSYM posreal_of_num_def, add_rzero, add_lzero]
+QED
 
 val preal_sub_eq = store_thm
   ("preal_sub_eq",
    ``!x y. preal x - preal y = if 0 <= y then preal (x - y) else preal x``,
    RW_TAC real_ss [preal_sub]
-   ++ RW_TAC real_ss [preal_def]
-   ++ MP_TAC (Q.SPEC `y` pos_def)
-   ++ DISCH_THEN (fn th => SIMP_TAC real_ss [th])
-   ++ RW_TAC std_ss []
-   ++ Know `0 = pos 0` >> RW_TAC real_ss [pos_def]
-   ++ DISCH_THEN (fn th => ONCE_REWRITE_TAC [th])
-   ++ RW_TAC std_ss [GSYM preal_def, GSYM posreal_of_num_def, sub_rzero]);
+   >> RW_TAC real_ss [preal_def]
+   >> MP_TAC (Q.SPEC `y` pos_def)
+   >> DISCH_THEN (fn th => SIMP_TAC real_ss [th])
+   >> RW_TAC std_ss []
+   >> Know `0 = pos 0` >- RW_TAC real_ss [pos_def]
+   >> DISCH_THEN (fn th => ONCE_REWRITE_TAC [th])
+   >> RW_TAC std_ss [GSYM preal_def, GSYM posreal_of_num_def, sub_rzero]);
 
 val preal_inj_eq = store_thm
   ("preal_inj_eq",
    ``!x y. (preal x = preal y) = if x <= 0 then y <= 0 else x = y``,
    RW_TAC real_ss [preal_def]
-   ++ REVERSE EQ_TAC >> METIS_TAC [REAL_POS_EQ_ZERO]
-   ++ STRIP_TAC
-   ++ Know `pos x = pos y`
-   >> METIS_TAC
-      [posreal_abs_inj, posreal_pred_def, REAL_POS_POS, optionTheory.SOME_11]
-   ++ POP_ASSUM (K ALL_TAC)
-   ++ METIS_TAC [REAL_POS_EQ_ZERO, pos_def]);
+   >> REVERSE EQ_TAC >- METIS_TAC [REAL_POS_EQ_ZERO]
+   >> STRIP_TAC
+   >> (Know `pos x = pos y`
+   >- METIS_TAC
+      [posreal_abs_inj, posreal_pred_def, REAL_POS_POS, optionTheory.SOME_11])
+   >> POP_ASSUM (K ALL_TAC)
+   >> METIS_TAC [REAL_POS_EQ_ZERO, pos_def]);
 
 val preal_le_eq = store_thm
   ("preal_le_eq",
-   ``!x y. preal x <= preal y = if 0 <= y then x <= y else x <= 0``,
-   RW_TAC real_ss [] >> METIS_TAC [preal_le, le_preal]
-   ++ Know `y <= 0` >> (POP_ASSUM MP_TAC ++ REAL_ARITH_TAC)
-   ++ RW_TAC real_ss [GSYM preal_eq_zero, le_zero]);
+   ``!x y. preal x <= preal y <=> if 0 <= y then x <= y else x <= 0``,
+   RW_TAC real_ss [] >- METIS_TAC [preal_le, le_preal]
+   >> Know `y <= 0` >- (POP_ASSUM MP_TAC >> REAL_ARITH_TAC)
+   >> RW_TAC real_ss [GSYM preal_eq_zero, le_zero]);
 
-val posreal_of_num_sub = store_thm
-  ("posreal_of_num_sub",
-   ``!m n : num. & m - & n = & (m - n)``,
-   RW_TAC real_ss [posreal_of_num_def, preal_sub]
-   ++ RW_TAC real_ss [preal_def]
-   ++ Suff `pos (& m - & n) = pos (& (m - n))` >> RW_TAC std_ss []
-   ++ REVERSE (Cases_on `0r <= & m - & n`)
-   >> (RW_TAC real_ss [pos_def]
-       ++ Suff `(& m : real) <= & n` >> RW_TAC real_ss []
-       ++ POP_ASSUM MP_TAC
-       ++ REAL_ARITH_TAC)
-   ++ RW_TAC real_ss [pos_def, REAL_EQ_SUB_RADD]
-   ++ Suff `n <= m` >> DECIDE_TAC
-   ++ Suff `(& n : real) <= & m` >> RW_TAC real_ss []
-   ++ POP_ASSUM MP_TAC
-   ++ REAL_ARITH_TAC);
+Theorem posreal_of_num_sub[allow_rebind]:
+  !m n : num. & m - & n = & (m - n)
+Proof
+  RW_TAC real_ss [posreal_of_num_def, preal_sub]
+  >> RW_TAC real_ss [preal_def]
+  >> Suff `pos (& m - & n) = pos (& (m - n))` >- RW_TAC std_ss []
+  >> REVERSE (Cases_on `0r <= & m - & n`)
+  >- (RW_TAC real_ss [pos_def]
+      >> Suff `(& m : real) <= & n` >- RW_TAC real_ss []
+      >> POP_ASSUM MP_TAC
+      >> REAL_ARITH_TAC)
+  >> RW_TAC real_ss [pos_def, REAL_EQ_SUB_RADD]
+  >> Suff `n <= m` >- DECIDE_TAC
+  >> Suff `(& n : real) <= & m` >- RW_TAC real_ss []
+  >> POP_ASSUM MP_TAC
+  >> REAL_ARITH_TAC
+QED
 
 val le_antisym_eq = store_thm
   ("le_antisym_eq",
-   ``!x y. (x = y) = x <= y /\ y <= x``,
+   ``!x y. x = y ⇔ x <= y /\ y <= x``,
    METIS_TAC [le_antisym, le_refl]);
 
 val add_sub = store_thm
   ("add_sub",
    ``!x y. ~(y = infty) ==> (x + y - y = x)``,
    REPEAT pcases
-   ++ RW_TAC real_ss
+   >> RW_TAC real_ss
       [preal_addr_def, preal_add_def, preal_subr_def, preal_sub_def,
        posreal_cancel, preal_not_infty, preal_def, infty_def, REAL_LE_ADD,
        pos_def]
-   ++ METIS_TAC [REAL_LE_ANTISYM, REAL_ADD_LID, REAL_LE_RADD]);
+   >> METIS_TAC [REAL_LE_ANTISYM, REAL_ADD_LID, REAL_LE_RADD]);
 
 val add_sub2 = store_thm
   ("add_sub2",
@@ -853,36 +850,36 @@ val le_sub_eq = store_thm
   ("le_sub_eq",
    ``!x y z.
        (~(y = 0) /\ (~(x = infty) \/ ~(z = infty))) ==>
-       (y <= z - x = y + x <= z)``,
+       (y <= z - x <=> y + x <= z)``,
    METIS_TAC [le_sub_imp, sub_lt_imp, preal_lt_def]);
 
 val sub_le_eq = store_thm
   ("sub_le_eq",
-   ``!x y z. (~(x = infty) \/ ~(y = infty)) ==> (y - x <= z = y <= z + x)``,
+   ``!x y z. (~(x = infty) \/ ~(y = infty)) ==> (y - x <= z ⇔ y <= z + x)``,
    METIS_TAC [sub_le_imp, lt_sub_imp, preal_lt_def]);
 
 val le_eq_sub_zero = store_thm
   ("le_eq_sub_zero",
-   ``!x y. x <= y = (y = infty) \/ (x - y = 0)``,
+   ``!x y. x <= y ⇔ (y = infty) \/ (x - y = 0)``,
    METIS_TAC [le_imp_sub_zero, sub_zero_imp_le, le_infty]);
 
 val mul_comm = store_thm
   ("mul_comm",
    ``!x y. x * y = y * x``,
    REPEAT pcases
-   ++ RW_TAC std_ss
+   >> RW_TAC std_ss
       [preal_mul_def, preal_mulr_def, posreal_cancel, infty_def, preal_def,
        REAL_POS_POS, posreal_of_num_def, pos_def]
-   ++ METIS_TAC [REAL_MUL_SYM]);
+   >> METIS_TAC [REAL_MUL_SYM]);
 
 val mul_assoc = store_thm
   ("mul_assoc",
    ``!x y z. x * y * z = x * (y * z)``,
    REPEAT pcases
-   ++ RW_TAC real_ss
+   >> RW_TAC real_ss
       [infty_def, preal_def, posreal_cancel, preal_mul_def, preal_mulr_def,
        REAL_LE_MUL]
-   ++ METIS_TAC
+   >> METIS_TAC
       [REAL_LE_ANTISYM, REAL_MUL_LZERO, pos_def, REAL_LE_REFL, REAL_ENTIRE,
        REAL_MUL_ASSOC]);
 
@@ -890,10 +887,10 @@ val mul_lzero = store_thm
   ("mul_lzero",
    ``!x. 0 * x = 0``,
    pcases
-   ++ RW_TAC std_ss
+   >> RW_TAC std_ss
       [preal_mul_def, preal_mulr_def, posreal_cancel, infty_def, preal_def,
        REAL_POS_POS, posreal_of_num_def]
-   ++ FULL_SIMP_TAC real_ss [pos_def]);
+   >> FULL_SIMP_TAC real_ss [pos_def]);
 
 val mul_rzero = store_thm
   ("mul_rzero",
@@ -904,11 +901,11 @@ val mul_linfty = store_thm
   ("mul_linfty",
    ``!x. infty * x = if x = 0 then 0 else infty``,
    RW_TAC std_ss [mul_rzero]
-   ++ pcases_on `x`
-   ++ RW_TAC std_ss
+   >> pcases_on `x`
+   >> RW_TAC std_ss
       [preal_mul_def, preal_mulr_def, posreal_cancel, infty_def, preal_def,
        REAL_POS_POS, posreal_of_num_def, pos_def]
-   ++ FULL_SIMP_TAC std_ss [posreal_of_num_def]);
+   >> FULL_SIMP_TAC std_ss [posreal_of_num_def]);
 
 val mul_rinfty = store_thm
   ("mul_rinfty",
@@ -919,10 +916,10 @@ val mul_lone = store_thm
   ("mul_lone",
    ``!x. 1 * x = x``,
    pcases
-   ++ RW_TAC real_ss
+   >> RW_TAC real_ss
       [posreal_of_num_def, preal_def, infty_def, preal_mul_def,
        posreal_cancel, REAL_POS_POS, preal_mulr_def]
-   ++ RW_TAC real_ss [pos_def]);
+   >> RW_TAC real_ss [pos_def]);
 
 val mul_rone = store_thm
   ("mul_rone",
@@ -931,22 +928,22 @@ val mul_rone = store_thm
 
 val entire = store_thm
   ("entire",
-   ``!x y. (x * y = 0) = (x = 0) \/ (y = 0)``,
+   ``!x y. x * y = 0 <=> x = 0 \/ y = 0``,
    REPEAT pcases3
-   ++ RW_TAC std_ss
+   >> RW_TAC std_ss
       [mul_lzero, mul_rzero, mul_linfty, posreal_of_num_not_infty, mul_rinfty,
        preal_mul]
-   ++ RW_TAC std_ss [posreal_of_num_def]
-   ++ METIS_TAC [preal_inj, REAL_ENTIRE, REAL_LE_REFL, REAL_LE_MUL]);
+   >> RW_TAC std_ss [posreal_of_num_def]
+   >> METIS_TAC [preal_inj, REAL_ENTIRE, REAL_LE_REFL, REAL_LE_MUL]);
 
 val le_mul2 = store_thm
   ("le_mul2",
    ``!x1 y1 x2 y2. x1 <= y1 /\ x2 <= y2 ==> x1 * x2 <= y1 * y2``,
    REPEAT pcases
-   ++ RW_TAC real_ss
+   >> RW_TAC real_ss
       [infty_def, preal_def, preal_mul_def, preal_mulr_def, preal_le_def,
        preal_ler_def, posreal_cancel, pos_def, REAL_LE_MUL]
-   ++ METIS_TAC
+   >> METIS_TAC
       [real_lt, REAL_LT_LE, REAL_MUL_RZERO, REAL_LE_ANTISYM, REAL_MUL_LZERO,
        REAL_LE_MUL2]);
 
@@ -960,27 +957,28 @@ val le_rmul_imp = store_thm
    ``!x y z. y <= z ==> y * x <= z * x``,
    METIS_TAC [le_lmul_imp, mul_comm]);
 
-val mul_eq_infty = store_thm
-  ("mul_eq_infty",
-   ``!x y.
-       (x * y = infty) = (x = infty) /\ ~(y = 0) \/ ~(x = 0) /\ (y = infty)``,
+Theorem mul_eq_infty:
+  !x y.
+    (x * y = infty) <=> (x = infty) /\ ~(y = 0) \/ ~(x = 0) /\ (y = infty)
+Proof
    pcases3
-   ++ pcases3
-   ++ RW_TAC std_ss [mul_linfty, mul_rinfty, mul_lzero, mul_rzero,
-                     posreal_of_num_not_infty, preal_mul, preal_not_infty]);
+   >> pcases3
+   >> RW_TAC std_ss [mul_linfty, mul_rinfty, mul_lzero, mul_rzero,
+                     posreal_of_num_not_infty, preal_mul, preal_not_infty]
+QED
 
 val add_ldistrib = store_thm
   ("add_ldistrib",
    ``!x y z. x * (y + z) = x * y + x * z``,
    REPEAT pcases3
-   ++ RW_TAC real_ss
+   >> RW_TAC real_ss
       [REAL_LE_ADD, REAL_LE_MUL, preal_mul, preal_add, mul_linfty,
        posreal_of_num_not_infty, add_linfty, add_rinfty, mul_rinfty,
        mul_lzero, add_lzero, mul_rzero, add_rzero, REAL_LDISTRIB]
-   ++ Suff `~(preal (y + y') = 0)` >> RW_TAC real_ss [mul_linfty]
-   ++ RW_TAC real_ss [preal_eq_zero]
-   ++ REPEAT (POP_ASSUM MP_TAC)
-   ++ REAL_ARITH_TAC);
+   >> Suff `~(preal (y + y') = 0)` >- RW_TAC real_ss [mul_linfty]
+   >> RW_TAC real_ss [preal_eq_zero]
+   >> REPEAT (POP_ASSUM MP_TAC)
+   >> REAL_ARITH_TAC);
 
 val add_rdistrib = store_thm
   ("add_rdistrib",
@@ -993,18 +991,18 @@ val sub_ldistrib = store_thm
        ~(x = infty) /\ (~(y = infty) \/ ~(z = infty)) ==>
        (x * (y - z) = x * y - x * z)``,
    RW_TAC std_ss []
-   ++ REVERSE (Cases_on `z <= y`)
-   >> (Know `y - z = 0` >> METIS_TAC [le_imp_sub_zero, le_total]
-       ++ RW_TAC std_ss [mul_rzero]
-       ++ METIS_TAC [le_total, le_imp_sub_zero, le_lmul_imp, mul_eq_infty])
-   ++ MATCH_MP_TAC le_antisym
-   ++ (CONJ_TAC
-       << [MATCH_MP_TAC le_sub_imp
-           ++ RW_TAC std_ss [mul_eq_infty, GSYM add_ldistrib]
-           ++ METIS_TAC [sub_add, infty_le, le_refl],
+   >> REVERSE (Cases_on `z <= y`)
+   >- (Know `y - z = 0` >- METIS_TAC [le_imp_sub_zero, le_total]
+       >> RW_TAC std_ss [mul_rzero]
+       >> METIS_TAC [le_total, le_imp_sub_zero, le_lmul_imp, mul_eq_infty])
+   >> MATCH_MP_TAC le_antisym
+   >> (CONJ_TAC
+       >| [MATCH_MP_TAC le_sub_imp
+           >> RW_TAC std_ss [mul_eq_infty, GSYM add_ldistrib]
+           >> METIS_TAC [sub_add, infty_le, le_refl],
            MATCH_MP_TAC sub_le_imp
-           ++ RW_TAC std_ss [mul_eq_infty, GSYM add_ldistrib]
-           ++ METIS_TAC [sub_add, infty_le, le_refl]]));
+           >> RW_TAC std_ss [mul_eq_infty, GSYM add_ldistrib]
+           >> METIS_TAC [sub_add, infty_le, le_refl]]));
 
 val sub_rdistrib = store_thm
   ("sub_rdistrib",
@@ -1021,8 +1019,8 @@ val mul_swap = store_thm
 val double = store_thm
   ("double",
    ``!x. 2 * x = x + x``,
-   Know `2 = 1 + 1` >> RW_TAC arith_ss [posreal_of_num_add, posreal_of_num_inj]
-   ++ RW_TAC std_ss [add_rdistrib, mul_lone]);
+   Know `2 = 1 + 1` >- RW_TAC arith_ss [posreal_of_num_add, posreal_of_num_inj]
+   >> RW_TAC std_ss [add_rdistrib, mul_lone]);
 
 val inv_zero = store_thm
   ("inv_zero",
@@ -1037,7 +1035,7 @@ val inv_infty = store_thm
    RW_TAC real_ss
    [posreal_of_num_def, preal_def, infty_def, preal_inv_def,
     posreal_cancel, REAL_POS_POS, preal_invr_def]
-   ++ RW_TAC real_ss [pos_def]);
+   >> RW_TAC real_ss [pos_def]);
 
 val inv_one = store_thm
   ("inv_one",
@@ -1045,7 +1043,7 @@ val inv_one = store_thm
    RW_TAC real_ss
    [posreal_of_num_def, preal_def, infty_def, preal_inv_def,
     posreal_cancel, REAL_POS_POS, preal_invr_def]
-   ++ RW_TAC real_ss [pos_def, REAL_INV1]);
+   >> RW_TAC real_ss [pos_def, REAL_INV1]);
 
 val preal_inv = store_thm
   ("preal_inv",
@@ -1053,51 +1051,52 @@ val preal_inv = store_thm
    RW_TAC real_ss
    [posreal_of_num_def, preal_def, infty_def, preal_inv_def,
     posreal_cancel, REAL_POS_POS, preal_invr_def]
-   << [METIS_TAC [REAL_LE_ANTISYM],
+   >| [METIS_TAC [REAL_LE_ANTISYM],
        METIS_TAC [REAL_LE_REFL],
        RW_TAC real_ss [pos_def, REAL_LE_INV]]);
 
-val inv_antimono = store_thm
-  ("inv_antimono",
-   ``!x y. inv x <= inv y = y <= x``,
+Theorem inv_antimono:
+  !x y. inv x <= inv y <=> y <= x
+Proof
    (REPEAT pcases3
-    ++ RW_TAC std_ss
+    >> RW_TAC std_ss
        [inv_zero, inv_infty, le_infty, zero_le, le_zero, preal_not_infty,
         posreal_of_num_inj, infty_le, posreal_of_num_not_infty, preal_inv])
-   >> (RW_TAC real_ss [posreal_of_num_def]
-       ++ METIS_TAC
+   >- (RW_TAC real_ss [posreal_of_num_def]
+       >> METIS_TAC
           [preal_inj, REAL_LE_INV, REAL_INV_EQ_0, pos_def, REAL_LE_REFL])
-   ++ Suff `~(inv y <= inv y') = ~(y' <= y)`
-   >> METIS_TAC [le_preal, preal_le, REAL_LE_INV]
-   ++ PURE_REWRITE_TAC [GSYM real_lt]
-   ++ MATCH_MP_TAC REAL_INV_LT_ANTIMONO
-   ++ REPEAT (Q.PAT_ASSUM `~(preal X = Y)` (K ALL_TAC))
-   ++ REPEAT (POP_ASSUM MP_TAC)
-   ++ REAL_ARITH_TAC);
+   >> Suff `~(inv y <= inv y') = ~(y' <= y)`
+   >- METIS_TAC [le_preal, preal_le, REAL_LE_INV]
+   >> PURE_REWRITE_TAC [GSYM real_lt]
+   >> MATCH_MP_TAC REAL_INV_LT_ANTIMONO
+   >> REPEAT (Q.PAT_X_ASSUM `~(preal X = Y)` (K ALL_TAC))
+   >> REPEAT (POP_ASSUM MP_TAC)
+   >> REAL_ARITH_TAC
+QED
 
 val inv_one_le = store_thm
   ("inv_one_le",
-   ``!x. 1 <= inv x = x <= 1``,
+   ``!x. 1 <= inv x <=> x <= 1``,
    ONCE_REWRITE_TAC [GSYM inv_one]
-   ++ RW_TAC std_ss [inv_antimono]
-   ++ RW_TAC std_ss [inv_one]);
+   >> RW_TAC std_ss [inv_antimono]
+   >> RW_TAC std_ss [inv_one]);
 
 val inv_le_one = store_thm
   ("inv_le_one",
-   ``!x. inv x <= 1 = 1 <= x``,
+   ``!x. inv x <= 1 <=> 1 <= x``,
    ONCE_REWRITE_TAC [GSYM inv_one]
-   ++ RW_TAC std_ss [inv_antimono]
-   ++ RW_TAC std_ss [inv_one]);
+   >> RW_TAC std_ss [inv_antimono]
+   >> RW_TAC std_ss [inv_one]);
 
 val inv_inv = store_thm
   ("inv_inv",
    ``!x. inv (inv x) = x``,
    pcases3
-   ++ RW_TAC std_ss [preal_not_infty, inv_zero, inv_infty]
-   ++ RW_TAC real_ss
+   >> RW_TAC std_ss [preal_not_infty, inv_zero, inv_infty]
+   >> RW_TAC real_ss
       [preal_inv_def, infty_def, preal_def, posreal_cancel, preal_invr_def,
        pos_def, REAL_LE_INV]
-   ++ METIS_TAC
+   >> METIS_TAC
       [REAL_INV_EQ_0, posreal_abs_inj, posreal_pred_def, REAL_LE_INV,
        optionTheory.SOME_11, REAL_INV_INV]);
 
@@ -1125,8 +1124,8 @@ val mul_linv = store_thm
   ("mul_linv",
    ``!x. ~(x = 0) /\ ~(x = infty) ==> (inv x * x = 1)``,
    pcases3
-   ++ RW_TAC std_ss [preal_not_infty]
-   ++ RW_TAC real_ss
+   >> RW_TAC std_ss [preal_not_infty]
+   >> RW_TAC real_ss
       [preal_inv_def, preal_mul_def, preal_def, preal_mulr_def,
        preal_invr_def, posreal_cancel, posreal_of_num_def, REAL_LE_INV,
        pos_def, REAL_MUL_LINV]);
@@ -1145,20 +1144,20 @@ val inv_mul = store_thm
   ("inv_mul",
    ``!a b. inv (a * b) = if a * b = 0 then infty else inv a * inv b``,
    pcases3
-   ++ pcases3
-   ++ RW_TAC std_ss
+   >> pcases3
+   >> RW_TAC std_ss
       [mul_linfty, mul_rinfty, mul_lzero, mul_rzero, inv_zero,
        posreal_of_num_not_infty, inv_infty, preal_mul]
-   ++ Know `0 <= y * y' /\ ~(y * y' = 0)`
-   >> METIS_TAC [REAL_ENTIRE, REAL_LE_MUL]
-   ++ RW_TAC std_ss [preal_inv, REAL_INV_MUL, REAL_LE_INV, preal_mul]);
+   >> Know `0 <= y * y' /\ ~(y * y' = 0)`
+   >- METIS_TAC [REAL_ENTIRE, REAL_LE_MUL]
+   >> RW_TAC std_ss [preal_inv, REAL_INV_MUL, REAL_LE_INV, preal_mul]);
 
 val half_between = store_thm
   ("half_between",
    ``(0 < 1/2 /\ 1/2 < 1) /\ (0 <= 1/2 /\ 1/2 <= 1)``,
    MATCH_MP_TAC (PROVE [] ``(x ==> y) /\ x ==> x /\ y``)
-   ++ CONJ_TAC >> PROVE_TAC [lt_le]
-   ++ SIMP_TAC arith_ss
+   >> CONJ_TAC >- PROVE_TAC [lt_le]
+   >> SIMP_TAC arith_ss
       [preal_div_def, mul_lone, preal_lt_def, le_zero, inv_eq_zero,
        posreal_of_num_not_infty, inv_one_le, posreal_of_num_le]);
 
@@ -1167,12 +1166,12 @@ val thirds_between = store_thm
    ``((0p < 1/3 /\ 1/3 < 1p) /\ (0p < 2/3 /\ 2/3 < 1p)) /\
      ((0p <= 1/3 /\ 1/3 <= 1p) /\ (0p <= 2/3 /\ 2/3 <= 1p))``,
    MATCH_MP_TAC (PROVE [] ``(x ==> y) /\ x ==> x /\ y``)
-   ++ CONJ_TAC >> PROVE_TAC [lt_le]
-   ++ RW_TAC real_ss
+   >> CONJ_TAC >- PROVE_TAC [lt_le]
+   >> RW_TAC real_ss
       [posreal_of_num_def, preal_lt_eq, preal_div_def, preal_mul, preal_inv,
        REAL_LE_INV, REAL_LE_MUL]
-   ++ RW_TAC std_ss [GSYM real_div]
-   ++ RW_TAC std_ss [REAL_INV_1OVER, REAL_THIRDS_BETWEEN]);
+   >> RW_TAC std_ss [GSYM real_div]
+   >> RW_TAC std_ss [REAL_INV_1OVER, REAL_THIRDS_BETWEEN]);
 
 val preal_div = store_thm
   ("preal_div",
@@ -1183,8 +1182,8 @@ val preal_div = store_thm
    RW_TAC std_ss
    [preal_div_def, preal_inv, mul_lzero, GSYM posreal_of_num_def,
     preal_mul, real_div, REAL_MUL_LZERO, mul_rinfty]
-   ++ RW_TAC real_ss [posreal_of_num_def]
-   ++ METIS_TAC [preal_inj]);
+   >> RW_TAC real_ss [posreal_of_num_def]
+   >> METIS_TAC [preal_inj]);
 
 val div_lzero = store_thm
   ("div_lzero",
@@ -1219,17 +1218,17 @@ val div_rinfty = store_thm
 
 val div_eq_zero = store_thm
   ("div_eq_zero",
-   ``!x y. (x / y = 0) = (x = 0) \/ (y = infty)``,
+   ``!x y. (x / y = 0) <=> (x = 0) \/ (y = infty)``,
    RW_TAC std_ss [preal_div_def, entire, inv_eq_zero]);
 
 val div_eq_infty = store_thm
   ("div_eq_infty",
    ``!x y.
-       (x / y = infty) =
+       (x / y = infty) <=>
        ~(x = 0) /\ (y = 0) \/
        (x = infty) /\ ~(y = infty)``,
    RW_TAC std_ss [preal_div_def, mul_eq_infty, inv_eq_zero, inv_eq_infty]
-   ++ METIS_TAC []);
+   >> METIS_TAC []);
 
 (* ------------------------------------------------------------------------- *)
 (* Minimum and maximum                                                       *)
@@ -1246,9 +1245,9 @@ val _ = overload_on ("max", Term `preal_max`);
 
 val min_le = store_thm
   ("min_le",
-   ``!z x y. min x y <= z = x <= z \/ y <= z``,
+   ``!z x y. min x y <= z <=> x <= z \/ y <= z``,
    RW_TAC std_ss [preal_min_def]
-   ++ PROVE_TAC [le_total, le_trans]);
+   >> PROVE_TAC [le_total, le_trans]);
 
 val min_le1 = store_thm
   ("min_le1",
@@ -1262,15 +1261,15 @@ val min_le2 = store_thm
 
 val le_min = store_thm
   ("le_min",
-   ``!z x y. z <= min x y = z <= x /\ z <= y``,
+   ``!z x y. z <= min x y <=> z <= x /\ z <= y``,
    RW_TAC std_ss [preal_min_def]
-   ++ PROVE_TAC [le_total, le_trans]);
+   >> PROVE_TAC [le_total, le_trans]);
 
 val min_le2_imp = store_thm
   ("min_le2_imp",
    ``!x1 x2 y1 y2. x1 <= y1 /\ x2 <= y2 ==> min x1 x2 <= min y1 y2``,
    RW_TAC std_ss [le_min]
-   ++ RW_TAC std_ss [min_le]);
+   >> RW_TAC std_ss [min_le]);
 
 val min_refl = store_thm
   ("min_refl",
@@ -1281,37 +1280,37 @@ val min_le_lin = store_thm
   ("min_le_lin",
    ``!z x y. min x y <= z * x + (1 - z) * y``,
    RW_TAC std_ss [preal_min_def]
-   << [MATCH_MP_TAC le_trans
-       ++ Cases_on `1 <= z`
-       >> (Q.EXISTS_TAC `z * x`
-           ++ RW_TAC std_ss [le_addr]
-           ++ METIS_TAC [le_rmul_imp, mul_lone])
-       ++ Q.EXISTS_TAC `z * x + (1 - z) * x`
-       ++ REVERSE CONJ_TAC >> RW_TAC std_ss [le_ladd, le_lmul_imp]
-       ++ RW_TAC std_ss [GSYM add_rdistrib]
-       ++ Know `z <= 1` >> METIS_TAC [le_total]
-       ++ STRIP_TAC
-       ++ Know `~(z = infty)` >> METIS_TAC [infty_le, posreal_of_num_not_infty]
-       ++ RW_TAC std_ss [sub_add2, mul_lone, le_refl],
-       Know `y <= x` >> METIS_TAC [le_total]
-       ++ STRIP_TAC
-       ++ MATCH_MP_TAC le_trans
-       ++ Q.EXISTS_TAC `z * y + (1 - z) * y`
-       ++ REVERSE CONJ_TAC >> RW_TAC std_ss [le_radd, le_lmul_imp]
-       ++ REVERSE (Cases_on `z <= 1`)
-       >> (MATCH_MP_TAC le_trans
-           ++ Q.EXISTS_TAC `z * y`
-           ++ RW_TAC std_ss [le_addr]
-           ++ METIS_TAC [le_rmul_imp, mul_lone, le_total])
-       ++ RW_TAC std_ss [GSYM add_rdistrib]
-       ++ Know `~(z = infty)` >> METIS_TAC [infty_le, posreal_of_num_not_infty]
-       ++ RW_TAC std_ss [sub_add2, mul_lone, le_refl]]);
+   >| [MATCH_MP_TAC le_trans
+       >> Cases_on `1 <= z`
+       >- (Q.EXISTS_TAC `z * x`
+           >> RW_TAC std_ss [le_addr]
+           >> METIS_TAC [le_rmul_imp, mul_lone])
+       >> Q.EXISTS_TAC `z * x + (1 - z) * x`
+       >> REVERSE CONJ_TAC >- RW_TAC std_ss [le_ladd, le_lmul_imp]
+       >> RW_TAC std_ss [GSYM add_rdistrib]
+       >> Know `z <= 1` >- METIS_TAC [le_total]
+       >> STRIP_TAC
+       >> Know `~(z = infty)` >- METIS_TAC [infty_le, posreal_of_num_not_infty]
+       >> RW_TAC std_ss [sub_add2, mul_lone, le_refl],
+       Know `y <= x` >- METIS_TAC [le_total]
+       >> STRIP_TAC
+       >> MATCH_MP_TAC le_trans
+       >> Q.EXISTS_TAC `z * y + (1 - z) * y`
+       >> REVERSE CONJ_TAC >- RW_TAC std_ss [le_radd, le_lmul_imp]
+       >> REVERSE (Cases_on `z <= 1`)
+       >- (MATCH_MP_TAC le_trans
+           >> Q.EXISTS_TAC `z * y`
+           >> RW_TAC std_ss [le_addr]
+           >> METIS_TAC [le_rmul_imp, mul_lone, le_total])
+       >> RW_TAC std_ss [GSYM add_rdistrib]
+       >> Know `~(z = infty)` >- METIS_TAC [infty_le, posreal_of_num_not_infty]
+       >> RW_TAC std_ss [sub_add2, mul_lone, le_refl]]);
 
 val min_comm = store_thm
   ("min_comm",
    ``!x y. min x y = min y x``,
    RW_TAC std_ss [preal_min_def]
-   ++ PROVE_TAC [le_antisym, le_total]);
+   >> PROVE_TAC [le_antisym, le_total]);
 
 val min_rinfty = store_thm
   ("min_rinfty",
@@ -1335,9 +1334,9 @@ val min_rzero = store_thm
 
 val le_max = store_thm
   ("le_max",
-   ``!z x y. z <= max x y = z <= x \/ z <= y``,
+   ``!z x y. z <= max x y <=> z <= x \/ z <= y``,
    RW_TAC std_ss [preal_max_def]
-   ++ PROVE_TAC [le_total, le_trans]);
+   >> PROVE_TAC [le_total, le_trans]);
 
 val le_max1 = store_thm
   ("le_max1",
@@ -1351,15 +1350,15 @@ val le_max2 = store_thm
 
 val max_le = store_thm
   ("max_le",
-   ``!z x y. max x y <= z = x <= z /\ y <= z``,
+   ``!z x y. max x y <= z <=> x <= z /\ y <= z``,
    RW_TAC std_ss [preal_max_def]
-   ++ PROVE_TAC [le_total, le_trans]);
+   >> PROVE_TAC [le_total, le_trans]);
 
 val max_le2_imp = store_thm
   ("max_le2_imp",
    ``!x1 x2 y1 y2. x1 <= y1 /\ x2 <= y2 ==> max x1 x2 <= max y1 y2``,
    RW_TAC std_ss [max_le]
-   ++ RW_TAC std_ss [le_max]);
+   >> RW_TAC std_ss [le_max]);
 
 val max_refl = store_thm
   ("max_refl",
@@ -1370,26 +1369,26 @@ val lin_le_max = store_thm
   ("lin_le_max",
    ``!z x y. z <= 1 ==> z * x + (1 - z) * y <= max x y``,
    RW_TAC std_ss [preal_max_def]
-   << [MATCH_MP_TAC le_trans
-       ++ Q.EXISTS_TAC `z * y + (1 - z) * y`
-       ++ CONJ_TAC >> RW_TAC std_ss [le_radd, le_lmul_imp]
-       ++ RW_TAC std_ss [GSYM add_rdistrib]
-       ++ Know `~(z = infty)` >> METIS_TAC [infty_le, posreal_of_num_not_infty]
-       ++ RW_TAC std_ss [sub_add2, mul_lone, le_refl],
-       Know `y <= x` >> METIS_TAC [le_total]
-       ++ STRIP_TAC
-       ++ MATCH_MP_TAC le_trans
-       ++ Q.EXISTS_TAC `z * x + (1 - z) * x`
-       ++ CONJ_TAC >> RW_TAC std_ss [le_ladd, le_lmul_imp]
-       ++ RW_TAC std_ss [GSYM add_rdistrib]
-       ++ Know `~(z = infty)` >> METIS_TAC [infty_le, posreal_of_num_not_infty]
-       ++ RW_TAC std_ss [sub_add2, mul_lone, le_refl]]);
+   >| [MATCH_MP_TAC le_trans
+       >> Q.EXISTS_TAC `z * y + (1 - z) * y`
+       >> CONJ_TAC >- RW_TAC std_ss [le_radd, le_lmul_imp]
+       >> RW_TAC std_ss [GSYM add_rdistrib]
+       >> Know `~(z = infty)` >- METIS_TAC [infty_le, posreal_of_num_not_infty]
+       >> RW_TAC std_ss [sub_add2, mul_lone, le_refl],
+       Know `y <= x` >- METIS_TAC [le_total]
+       >> STRIP_TAC
+       >> MATCH_MP_TAC le_trans
+       >> Q.EXISTS_TAC `z * x + (1 - z) * x`
+       >> CONJ_TAC >- RW_TAC std_ss [le_ladd, le_lmul_imp]
+       >> RW_TAC std_ss [GSYM add_rdistrib]
+       >> Know `~(z = infty)` >- METIS_TAC [infty_le, posreal_of_num_not_infty]
+       >> RW_TAC std_ss [sub_add2, mul_lone, le_refl]]);
 
 val max_comm = store_thm
   ("max_comm",
    ``!x y. max x y = max y x``,
    RW_TAC std_ss [preal_max_def]
-   ++ PROVE_TAC [le_antisym, le_total]);
+   >> PROVE_TAC [le_antisym, le_total]);
 
 val max_rinfty = store_thm
   ("max_rinfty",
@@ -1432,9 +1431,9 @@ val bound1_cancel = store_thm
   ("bound1_cancel",
    ``!x. bound1 x + (1 - bound1 x) = 1``,
    GEN_TAC
-   ++ MATCH_MP_TAC sub_add2
-   ++ RW_TAC std_ss [bound1]
-   ++ METIS_TAC [posreal_of_num_not_infty, infty_le, le_trans, bound1]);
+   >> MATCH_MP_TAC sub_add2
+   >> RW_TAC std_ss [bound1]
+   >> METIS_TAC [posreal_of_num_not_infty, infty_le, le_trans, bound1]);
 
 val bound1_cancel2 = store_thm
   ("bound1_cancel2",
@@ -1472,97 +1471,95 @@ val le_sup_imp = store_thm
   ("le_sup_imp",
    ``!p x. p x ==> x <= sup p``,
    RW_TAC std_ss [preal_sup_def, le_infty]
-   ++ FULL_SIMP_TAC std_ss []
-   ++ Know `~p infty` >> METIS_TAC [infty_le]
-   ++ STRIP_TAC
-   ++ pcases_on `x`
-   ++ MATCH_MP_TAC preal_le
-   ++ RW_TAC real_ss []
-   ++ pcases_on `x'`
-   ++ MATCH_MP_TAC REAL_IMP_LE_SUP
-   ++ CONJ_TAC >> METIS_TAC []
-   ++ REVERSE CONJ_TAC >> (Q.EXISTS_TAC `y` ++ RW_TAC real_ss [])
-   ++ Q.EXISTS_TAC `y'`
-   ++ RW_TAC std_ss []
-   ++ RW_TAC std_ss []
-   ++ MATCH_MP_TAC le_preal
-   ++ METIS_TAC []);
+   >> FULL_SIMP_TAC std_ss []
+   >> Know `~p infty` >- METIS_TAC [infty_le]
+   >> STRIP_TAC
+   >> pcases_on `x`
+   >> MATCH_MP_TAC preal_le
+   >> RW_TAC real_ss []
+   >> pcases_on `x'`
+   >> MATCH_MP_TAC REAL_IMP_LE_SUP
+   >> REVERSE CONJ_TAC >- (Q.EXISTS_TAC `y` >> RW_TAC real_ss [])
+   >> Q.EXISTS_TAC `y'`
+   >> RW_TAC std_ss []
+   >> RW_TAC std_ss []
+   >> MATCH_MP_TAC le_preal
+   >> METIS_TAC []);
 
 val sup_le = store_thm
   ("sup_le",
-   ``!p x. sup p <= x = (!y. p y ==> y <= x)``,
+   ``!p x. sup p <= x <=> (!y. p y ==> y <= x)``,
    RW_TAC std_ss [preal_sup_def, infty_le]
-   >> (EQ_TAC >> RW_TAC std_ss [le_infty] ++ METIS_TAC [])
-   ++ FULL_SIMP_TAC std_ss []
-   ++ Know `~p infty` >> METIS_TAC [infty_le]
-   ++ STRIP_TAC
-   ++ pcases_on `x` >> RW_TAC std_ss [le_infty]
-   ++ pcases_on `x'`
-   ++ EQ_TAC
-   << [RW_TAC std_ss []
-       ++ pcases_on `y''`
-       ++ MATCH_MP_TAC le_trans
-       ++ Q.EXISTS_TAC `preal (sup (\r. (r = 0) \/ 0 <= r /\ p (preal r)))`
-       ++ RW_TAC std_ss []
-       ++ MATCH_MP_TAC preal_le
-       ++ MATCH_MP_TAC REAL_IMP_LE_SUP
-       ++ CONJ_TAC >> METIS_TAC []
-       ++ REVERSE CONJ_TAC >> (Q.EXISTS_TAC `y'''` ++ RW_TAC real_ss [])
-       ++ Q.EXISTS_TAC `y'`
-       ++ RW_TAC std_ss []
-       ++ RW_TAC std_ss []
-       ++ METIS_TAC [le_preal],
+   >- (EQ_TAC >- RW_TAC std_ss [le_infty] >> METIS_TAC [])
+   >> FULL_SIMP_TAC std_ss []
+   >> Know `~p infty` >- METIS_TAC [infty_le]
+   >> STRIP_TAC
+   >> pcases_on `x` >- RW_TAC std_ss [le_infty]
+   >> pcases_on `x'`
+   >> EQ_TAC
+   >| [RW_TAC std_ss []
+       >> pcases_on `y''`
+       >> MATCH_MP_TAC le_trans
+       >> Q.EXISTS_TAC `preal (sup (\r. (r = 0) \/ 0 <= r /\ p (preal r)))`
+       >> RW_TAC std_ss []
+       >> MATCH_MP_TAC preal_le
+       >> MATCH_MP_TAC REAL_IMP_LE_SUP
+       >> REVERSE CONJ_TAC >- (Q.EXISTS_TAC `y'''` >> RW_TAC real_ss [])
+       >> Q.EXISTS_TAC `y'`
+       >> RW_TAC std_ss []
+       >> RW_TAC std_ss []
+       >> METIS_TAC [le_preal],
        RW_TAC std_ss []
-       ++ MATCH_MP_TAC preal_le
-       ++ MATCH_MP_TAC REAL_IMP_SUP_LE
-       ++ CONJ_TAC >> METIS_TAC []
-       ++ RW_TAC std_ss []
-       ++ RW_TAC std_ss []
-       ++ MATCH_MP_TAC le_preal
-       ++ RW_TAC std_ss []]);
+       >> MATCH_MP_TAC preal_le
+       >> MATCH_MP_TAC REAL_IMP_SUP_LE
+       >> CONJ_TAC >- METIS_TAC []
+       >> RW_TAC std_ss []
+       >> RW_TAC std_ss []
+       >> MATCH_MP_TAC le_preal
+       >> RW_TAC std_ss []]);
 
 val le_sup = store_thm
   ("le_sup",
-   ``!p x. x <= sup p = !y. (!z. p z ==> z <= y) ==> x <= y``,
+   ``!p x. x <= sup p <=> !y. (!z. p z ==> z <= y) ==> x <= y``,
    RW_TAC std_ss [preal_sup_def, le_infty]
-   ++ FULL_SIMP_TAC std_ss []
-   ++ pcases_on `x'`
-   ++ Q.PAT_ASSUM `~X` (K ALL_TAC)
-   ++ pcases_on `x`
-   >> (RW_TAC std_ss [infty_le, preal_not_infty]
-       ++ Q.EXISTS_TAC `preal y`
-       ++ RW_TAC std_ss [preal_not_infty])
-   ++ ASM_SIMP_TAC real_ss [preal_le_eq]
-   ++ MATCH_MP_TAC (PROVE [] ``x /\ (y = z) ==> ((if x then y else w) = z)``)
-   ++ CONJ_TAC
-   >> (RW_TAC std_ss []
-       ++ MATCH_MP_TAC REAL_IMP_LE_SUP
-       ++ METIS_TAC [REAL_LE_REFL, le_preal])
-   ++ MP_TAC
+   >> FULL_SIMP_TAC std_ss []
+   >> pcases_on `x'`
+   >> Q.PAT_X_ASSUM `~X` (K ALL_TAC)
+   >> pcases_on `x`
+   >- (RW_TAC std_ss [infty_le, preal_not_infty]
+       >> Q.EXISTS_TAC `preal y`
+       >> RW_TAC std_ss [preal_not_infty])
+   >> ASM_SIMP_TAC real_ss [preal_le_eq]
+   >> MATCH_MP_TAC (PROVE [] ``x /\ (y = z) ==> ((if x then y else w) = z)``)
+   >> CONJ_TAC
+   >- (RW_TAC std_ss []
+       >> MATCH_MP_TAC REAL_IMP_LE_SUP
+       >> METIS_TAC [REAL_LE_REFL, le_preal])
+   >> MP_TAC
       (Q.SPECL [`\r. (r = 0) \/ 0 <= r /\ p (preal r)`, `y'`] REAL_LE_SUP)
-   ++ MATCH_MP_TAC (PROVE [] ``x /\ (y ==> z) ==> (x ==> y) ==> z``)
-   ++ CONJ_TAC >> METIS_TAC [le_preal]
-   ++ DISCH_THEN (fn th => REWRITE_TAC [th])
-   ++ RW_TAC std_ss []
-   ++ EQ_TAC
-   << [RW_TAC std_ss []
-       ++ pcases_on `y''` >> RW_TAC std_ss [le_infty]
-       ++ MATCH_MP_TAC preal_le
-       ++ Q.PAT_ASSUM (`!a. (!b. P a b) ==> Q a`) MATCH_MP_TAC
-       ++ METIS_TAC [le_preal, preal_le],
+   >> MATCH_MP_TAC (PROVE [] ``x /\ (y ==> z) ==> (x ==> y) ==> z``)
+   >> CONJ_TAC >- METIS_TAC [le_preal]
+   >> DISCH_THEN (fn th => REWRITE_TAC [th])
+   >> RW_TAC std_ss []
+   >> EQ_TAC
+   >| [RW_TAC std_ss []
+       >> pcases_on `y''` >- RW_TAC std_ss [le_infty]
+       >> MATCH_MP_TAC preal_le
+       >> Q.PAT_X_ASSUM (`!a. (!b. P a b) ==> Q a`) MATCH_MP_TAC
+       >> METIS_TAC [le_preal, preal_le],
        RW_TAC std_ss []
-       ++ MATCH_MP_TAC le_preal
-       ++ RW_TAC std_ss []
-       ++ FIRST_ASSUM MATCH_MP_TAC
-       ++ RW_TAC std_ss []
-       ++ pcases_on `z` >> METIS_TAC [infty_le, preal_not_infty]
-       ++ MATCH_MP_TAC preal_le
-       ++ METIS_TAC [le_preal, preal_le]]);
+       >> MATCH_MP_TAC le_preal
+       >> RW_TAC std_ss []
+       >> FIRST_ASSUM MATCH_MP_TAC
+       >> RW_TAC std_ss []
+       >> pcases_on `z` >- METIS_TAC [infty_le, preal_not_infty]
+       >> MATCH_MP_TAC preal_le
+       >> METIS_TAC [le_preal, preal_le]]);
 
 val sup_eq = store_thm
   ("sup_eq",
    ``!p x.
-       (sup p = x) =
+       (sup p = x) <=>
        (!y. p y ==> y <= x) /\ !y. (!z. p z ==> z <= y) ==> x <= y``,
    RW_TAC std_ss [le_antisym_eq, le_sup, sup_le]);
 
@@ -1575,15 +1572,15 @@ val sup_num = store_thm
   ("sup_num",
    ``sup (\x. ?n : num. x = & n) = infty``,
    MATCH_MP_TAC le_antisym
-   ++ RW_TAC std_ss [le_infty, le_sup]
-   ++ pcases_on `y` >> RW_TAC std_ss [le_refl]
-   ++ RW_TAC std_ss [infty_le, preal_not_infty]
-   ++ MP_TAC (Q.SPEC `y'` REAL_BIGNUM)
-   ++ PURE_REWRITE_TAC [real_lt]
-   ++ STRIP_TAC
-   ++ Q.PAT_ASSUM `!z. P z` (MP_TAC o Q.SPEC `&n`)
-   ++ RW_TAC std_ss [posreal_of_num_def] >> METIS_TAC []
-   ++ METIS_TAC [le_preal]);
+   >> RW_TAC std_ss [le_infty, le_sup]
+   >> pcases_on `y` >- RW_TAC std_ss [le_refl]
+   >> RW_TAC std_ss [infty_le, preal_not_infty]
+   >> MP_TAC (Q.SPEC `y'` REAL_BIGNUM)
+   >> PURE_REWRITE_TAC [real_lt]
+   >> STRIP_TAC
+   >> Q.PAT_X_ASSUM `!z. P z` (MP_TAC o Q.SPEC `&n`)
+   >> RW_TAC std_ss [posreal_of_num_def] >- METIS_TAC []
+   >> METIS_TAC [le_preal]);
 
 val sup_rmult = store_thm
   ("sup_rmult",
@@ -1591,33 +1588,33 @@ val sup_rmult = store_thm
        sup (\y. ?z : 'a. p z /\ (y = f z * x)) =
        sup (\y. ?z. p z /\ (y = f z)) * x``,
    REPEAT GEN_TAC
-   ++ Cases_on `x = 0`
-   >> RW_TAC real_ss [mul_rzero, GSYM le_zero, sup_le, le_refl]
-   ++ MATCH_MP_TAC le_antisym
-   ++ RW_TAC real_ss [sup_le, le_sup]
-   >> (MATCH_MP_TAC le_rmul_imp ++ RW_TAC std_ss [le_sup] ++ METIS_TAC [])
-   ++ REVERSE (Cases_on `?x. p x`)
-   >> (Suff `sup (\y. ?z. p z /\ (y = f z)) = 0`
-       >> RW_TAC real_ss [mul_lzero, zero_le]
-       ++ RW_TAC std_ss [GSYM le_zero, sup_le]
-       ++ METIS_TAC [])
-   ++ Cases_on `x = infty`
-   >> (Cases_on `!z. p z ==> (f z = 0)`
-       >> (Suff `sup (\y. ?z. p z /\ (y = f z)) = 0`
-           >> RW_TAC real_ss [mul_lzero, zero_le]
-           ++ RW_TAC std_ss [GSYM le_zero, sup_le]
-           ++ METIS_TAC [le_zero])
-       ++ FULL_SIMP_TAC std_ss []
-       ++ Suff `infty <= y` >> RW_TAC real_ss [infty_le, le_infty]
-       ++ Q.PAT_ASSUM `!z. P z` MATCH_MP_TAC
-       ++ METIS_TAC [mul_rinfty])
-   ++ Suff `sup (\y. ?z. p z /\ (y = f z)) * x <= (y * inv x) * x`
-   >> RW_TAC real_ss [mul_assoc, mul_linv, mul_rone]
-   ++ MATCH_MP_TAC le_rmul_imp
-   ++ RW_TAC real_ss [sup_le]
-   ++ Suff `(f z * x) * inv x <= y * inv x`
-   >> RW_TAC real_ss [mul_assoc, mul_rinv, mul_rone]
-   ++ METIS_TAC [le_rmul_imp]);
+   >> Cases_on `x = 0`
+   >- RW_TAC real_ss [mul_rzero, GSYM le_zero, sup_le, le_refl]
+   >> MATCH_MP_TAC le_antisym
+   >> RW_TAC real_ss [sup_le, le_sup]
+   >- (MATCH_MP_TAC le_rmul_imp >> RW_TAC std_ss [le_sup] >> METIS_TAC [])
+   >> REVERSE (Cases_on `?x. p x`)
+   >- (Suff `sup (\y. ?z. p z /\ (y = f z)) = 0`
+       >- RW_TAC real_ss [mul_lzero, zero_le]
+       >> RW_TAC std_ss [GSYM le_zero, sup_le]
+       >> METIS_TAC [])
+   >> Cases_on `x = infty`
+   >- (Cases_on `!z. p z ==> (f z = 0)`
+       >- (Suff `sup (\y. ?z. p z /\ (y = f z)) = 0`
+           >- RW_TAC real_ss [mul_lzero, zero_le]
+           >> RW_TAC std_ss [GSYM le_zero, sup_le]
+           >> METIS_TAC [le_zero])
+       >> FULL_SIMP_TAC std_ss []
+       >> Suff `infty <= y` >- RW_TAC real_ss [infty_le, le_infty]
+       >> Q.PAT_X_ASSUM `!z. P z` MATCH_MP_TAC
+       >> METIS_TAC [mul_rinfty])
+   >> Suff `sup (\y. ?z. p z /\ (y = f z)) * x <= (y * inv x) * x`
+   >- RW_TAC real_ss [mul_assoc, mul_linv, mul_rone]
+   >> MATCH_MP_TAC le_rmul_imp
+   >> RW_TAC real_ss [sup_le]
+   >> Suff `(f z * x) * inv x <= y * inv x`
+   >- RW_TAC real_ss [mul_assoc, mul_rinv, mul_rone]
+   >> METIS_TAC [le_rmul_imp]);
 
 val sup_lmult = store_thm
   ("sup_lmult",
@@ -1625,23 +1622,23 @@ val sup_lmult = store_thm
        sup (\y. ?z : 'a. p z /\ (y = x * f z)) =
        x * sup (\y. ?z. p z /\ (y = f z))``,
    ONCE_REWRITE_TAC [mul_comm]
-   ++ RW_TAC std_ss [sup_rmult]);
+   >> RW_TAC std_ss [sup_rmult]);
 
 val sup_rmul = store_thm
   ("sup_rmul",
    ``!f x. sup (\y. ?z : 'a. y = f z * x) = sup (\y. ?z. y = f z) * x``,
    REPEAT GEN_TAC
-   ++ Suff
+   >> Suff
       `sup (\y. ?z : 'a. T /\ (y = f z * x)) = sup (\y. ?z. T /\ (y = f z)) * x`
-   >> RW_TAC std_ss []
-   ++ SIMP_TAC pureSimps.pure_ss [sup_rmult]
-   ++ RW_TAC std_ss []);
+   >- RW_TAC std_ss []
+   >> SIMP_TAC pureSimps.pure_ss [sup_rmult]
+   >> RW_TAC std_ss []);
 
 val sup_lmul = store_thm
   ("sup_lmul",
    ``!f x. sup (\y. ?z : 'a. y = x * f z) = x * sup (\y. ?z. y = f z)``,
    ONCE_REWRITE_TAC [mul_comm]
-   ++ RW_TAC std_ss [sup_rmul]);
+   >> RW_TAC std_ss [sup_rmul]);
 
 val sup_num_mul = store_thm
   ("sup_num_mul",
@@ -1654,113 +1651,113 @@ val add_sup = store_thm
        sup p + sup q =
        sup (\r. ?x y. (p x \/ (x = 0)) /\ (q y \/ (y = 0)) /\ (r = x + y))``,
    RW_TAC std_ss []
-   ++ MATCH_MP_TAC EQ_SYM
-   ++ REWRITE_TAC [sup_eq]
-   ++ CONJ_TAC
-   >> (RW_TAC std_ss []
-       ++ MATCH_MP_TAC le_add2
-       ++ RW_TAC std_ss [le_sup_imp, zero_le])
-   ++ RW_TAC std_ss []
-   ++ Cases_on `y = infty` >> RW_TAC std_ss [le_infty]
-   ++ Cases_on `sup p = 0` >> RW_TAC std_ss [sup_le, add_lzero]
-   ++ Cases_on `sup q = 0` >> RW_TAC std_ss [sup_le, add_rzero]
-   ++ MATCH_MP_TAC le_trans
-   ++ Q.EXISTS_TAC `sup (\r. ?y. (q y \/ (y = 0)) /\ (r = sup p + y))`
-   ++ REVERSE CONJ_TAC
-   >> (REVERSE (RW_TAC std_ss [sup_le]) >> RW_TAC std_ss [sup_le, add_rzero]
-       ++ Suff `sup p <= y - y'` >> RW_TAC std_ss [le_sub_eq]
-       ++ RW_TAC std_ss [sup_le]
-       ++ MATCH_MP_TAC le_sub_imp
-       ++ RW_TAC std_ss []
-       ++ METIS_TAC [])
-   ++ Cases_on `sup p = infty`
-   >> (RW_TAC std_ss [add_linfty]
-       ++ Know `!r. (?y'. (q y' \/ (y' = 0)) /\ (r = infty)) = (r = infty)`
-       >> METIS_TAC []
-       ++ RW_TAC std_ss [sup_const, le_refl])
-   ++ ONCE_REWRITE_TAC [add_comm]
-   ++ Suff `sup q <= sup (\r. ?y. (q y \/ (y = 0)) /\ (r = y + sup p)) - sup p`
-   >> RW_TAC std_ss [le_sub_eq]
-   ++ RW_TAC std_ss [sup_le]
-   ++ MATCH_MP_TAC le_sub_imp
-   ++ RW_TAC std_ss []
-   ++ RW_TAC std_ss [le_sup]
-   ++ METIS_TAC []);
+   >> MATCH_MP_TAC EQ_SYM
+   >> REWRITE_TAC [sup_eq]
+   >> CONJ_TAC
+   >- (RW_TAC std_ss []
+       >> MATCH_MP_TAC le_add2
+       >> RW_TAC std_ss [le_sup_imp, zero_le])
+   >> RW_TAC std_ss []
+   >> Cases_on `y = infty` >- RW_TAC std_ss [le_infty]
+   >> Cases_on `sup p = 0` >- RW_TAC std_ss [sup_le, add_lzero]
+   >> Cases_on `sup q = 0` >- RW_TAC std_ss [sup_le, add_rzero]
+   >> MATCH_MP_TAC le_trans
+   >> Q.EXISTS_TAC `sup (\r. ?y. (q y \/ (y = 0)) /\ (r = sup p + y))`
+   >> REVERSE CONJ_TAC
+   >- (REVERSE (RW_TAC std_ss [sup_le]) >- RW_TAC std_ss [sup_le, add_rzero]
+       >> Suff `sup p <= y - y'` >- RW_TAC std_ss [le_sub_eq]
+       >> RW_TAC std_ss [sup_le]
+       >> MATCH_MP_TAC le_sub_imp
+       >> RW_TAC std_ss []
+       >> METIS_TAC [])
+   >> Cases_on `sup p = infty`
+   >- (RW_TAC std_ss [add_linfty]
+       >> Know `!r. (?y'. (q y' \/ (y' = 0)) /\ (r = infty)) = (r = infty)`
+       >- METIS_TAC []
+       >> RW_TAC std_ss [sup_const, le_refl])
+   >> ONCE_REWRITE_TAC [add_comm]
+   >> Suff `sup q <= sup (\r. ?y. (q y \/ (y = 0)) /\ (r = y + sup p)) - sup p`
+   >- RW_TAC std_ss [le_sub_eq]
+   >> RW_TAC std_ss [sup_le]
+   >> MATCH_MP_TAC le_sub_imp
+   >> RW_TAC std_ss []
+   >> RW_TAC std_ss [le_sup]
+   >> METIS_TAC []);
 
 val sup_le_sup_imp = store_thm
   ("sup_le_sup_imp",
    ``!p q. (!x. p x ==> ?y. q y /\ x <= y) ==> sup p <= sup q``,
-   RW_TAC std_ss [sup_le] ++ METIS_TAC [le_trans, le_sup_imp]);
+   RW_TAC std_ss [sup_le] >> METIS_TAC [le_trans, le_sup_imp]);
 
 val inf_le_imp = store_thm
   ("inf_le_imp",
    ``!p x. p x ==> inf p <= x``,
    RW_TAC std_ss [preal_inf_def, le_infty]
-   ++ FULL_SIMP_TAC std_ss []
-   ++ pcases_on `x` >> RW_TAC std_ss [le_infty]
-   ++ MATCH_MP_TAC preal_le
-   ++ MATCH_MP_TAC REAL_IMP_INF_LE
-   ++ CONJ_TAC >> METIS_TAC []
-   ++ METIS_TAC [REAL_LE_REFL]);
+   >> FULL_SIMP_TAC std_ss []
+   >> pcases_on `x` >- RW_TAC std_ss [le_infty]
+   >> MATCH_MP_TAC preal_le
+   >> MATCH_MP_TAC REAL_IMP_INF_LE
+   >> CONJ_TAC >- METIS_TAC []
+   >> METIS_TAC [REAL_LE_REFL]);
 
 val le_inf = store_thm
   ("le_inf",
-   ``!p x. x <= inf p = (!y. p y ==> x <= y)``,
+   ``!p x. x <= inf p <=> (!y. p y ==> x <= y)``,
    RW_TAC std_ss [preal_inf_def, le_infty]
-   ++ FULL_SIMP_TAC std_ss []
-   ++ pcases_on `x'`
-   ++ pcases_on `x`
-   >> (RW_TAC std_ss [infty_le]
-       ++ MATCH_MP_TAC (PROVE [] ``~x /\ ~y ==> (x = y)``)
-       ++ REVERSE CONJ_TAC >> METIS_TAC []
-       ++ METIS_TAC [preal_not_infty])
-   ++ EQ_TAC
-   << [RW_TAC std_ss []
-       ++ pcases_on `y''` >> RW_TAC std_ss [le_infty]
-       ++ MATCH_MP_TAC le_trans
-       ++ Q.EXISTS_TAC `preal (inf (\r. 0 <= r /\ p (preal r)))`
-       ++ RW_TAC std_ss []
-       ++ MATCH_MP_TAC preal_le
-       ++ MATCH_MP_TAC REAL_IMP_INF_LE
-       ++ CONJ_TAC >> METIS_TAC []
-       ++ METIS_TAC [REAL_LE_REFL],
+   >> FULL_SIMP_TAC std_ss []
+   >> pcases_on `x'`
+   >> pcases_on `x`
+   >- (RW_TAC std_ss [infty_le]
+       >> MATCH_MP_TAC (PROVE [] ``~x /\ ~y ==> (x = y)``)
+       >> REVERSE CONJ_TAC >- METIS_TAC []
+       >> METIS_TAC [preal_not_infty])
+   >> EQ_TAC
+   >| [RW_TAC std_ss []
+       >> pcases_on `y''` >- RW_TAC std_ss [le_infty]
+       >> MATCH_MP_TAC le_trans
+       >> Q.EXISTS_TAC `preal (inf (\r. 0 <= r /\ p (preal r)))`
+       >> RW_TAC std_ss []
+       >> MATCH_MP_TAC preal_le
+       >> MATCH_MP_TAC REAL_IMP_INF_LE
+       >> CONJ_TAC >- METIS_TAC []
+       >> METIS_TAC [REAL_LE_REFL],
        RW_TAC std_ss []
-       ++ MATCH_MP_TAC preal_le
-       ++ MATCH_MP_TAC REAL_IMP_LE_INF
-       ++ CONJ_TAC >> METIS_TAC []
-       ++ RW_TAC std_ss []
-       ++ MATCH_MP_TAC le_preal
-       ++ RW_TAC std_ss []]);
+       >> MATCH_MP_TAC preal_le
+       >> MATCH_MP_TAC REAL_IMP_LE_INF
+       >> CONJ_TAC >- METIS_TAC []
+       >> RW_TAC std_ss []
+       >> MATCH_MP_TAC le_preal
+       >> RW_TAC std_ss []]);
 
 val inf_le = store_thm
   ("inf_le",
-   ``!p x. inf p <= x = !y. (!z. p z ==> y <= z) ==> y <= x``,
-   RW_TAC std_ss [preal_inf_def, le_infty] >> METIS_TAC [infty_le, le_infty]
-   ++ FULL_SIMP_TAC std_ss []
-   ++ pcases_on `x'`
-   ++ Q.PAT_ASSUM `~X` (K ALL_TAC)
-   ++ pcases_on `x` >> RW_TAC std_ss [infty_le, preal_not_infty, le_infty]
-   ++ RW_TAC real_ss [preal_le_eq]
-   ++ MP_TAC
+   ``!p x. inf p <= x <=> !y. (!z. p z ==> y <= z) ==> y <= x``,
+   RW_TAC std_ss [preal_inf_def, le_infty] >- METIS_TAC [infty_le, le_infty]
+   >> FULL_SIMP_TAC std_ss []
+   >> pcases_on `x'`
+   >> Q.PAT_X_ASSUM `~X` (K ALL_TAC)
+   >> pcases_on `x` >- RW_TAC std_ss [infty_le, preal_not_infty, le_infty]
+   >> RW_TAC real_ss [preal_le_eq]
+   >> MP_TAC
       (Q.SPECL [`\r. 0 <= r /\ p (preal r)`, `y'`] REAL_INF_LE)
-   ++ MATCH_MP_TAC (PROVE [] ``x /\ (y ==> z) ==> (x ==> y) ==> z``)
-   ++ CONJ_TAC >> METIS_TAC [le_preal]
-   ++ DISCH_THEN (fn th => REWRITE_TAC [th])
-   ++ RW_TAC std_ss []
-   ++ EQ_TAC
-   << [RW_TAC std_ss []
-       ++ pcases_on `y''` >> METIS_TAC [infty_le, preal_not_infty]
-       ++ MATCH_MP_TAC preal_le
-       ++ Q.PAT_ASSUM (`!a. (!b. P a b) ==> Q a`) MATCH_MP_TAC
-       ++ METIS_TAC [le_preal, preal_le],
+   >> MATCH_MP_TAC (PROVE [] ``x /\ (y ==> z) ==> (x ==> y) ==> z``)
+   >> CONJ_TAC >- METIS_TAC [le_preal]
+   >> DISCH_THEN (fn th => REWRITE_TAC [th])
+   >> RW_TAC std_ss []
+   >> EQ_TAC
+   >| [RW_TAC std_ss []
+       >> pcases_on `y''` >- METIS_TAC [infty_le, preal_not_infty]
+       >> MATCH_MP_TAC preal_le
+       >> Q.PAT_X_ASSUM (`!a. (!b. P a b) ==> Q a`) MATCH_MP_TAC
+       >> METIS_TAC [le_preal, preal_le],
        RW_TAC std_ss []
-       ++ MATCH_MP_TAC le_preal
-       ++ RW_TAC std_ss []
-       ++ FIRST_ASSUM MATCH_MP_TAC
-       ++ RW_TAC std_ss []
-       ++ pcases_on `z` >> RW_TAC std_ss [le_infty]
-       ++ MATCH_MP_TAC preal_le
-       ++ METIS_TAC [le_preal, preal_le]]);
+       >> MATCH_MP_TAC le_preal
+       >> RW_TAC std_ss []
+       >> FIRST_ASSUM MATCH_MP_TAC
+       >> RW_TAC std_ss []
+       >> pcases_on `z` >- RW_TAC std_ss [le_infty]
+       >> MATCH_MP_TAC preal_le
+       >> METIS_TAC [le_preal, preal_le]]);
 
 (* ------------------------------------------------------------------------- *)
 (* (posreal,<=) is a complete lattice                                        *)
@@ -1782,7 +1779,7 @@ val posreal_complete = store_thm
   ("posreal_complete",
    ``complete (posreal, (<=))``,
    RW_TAC std_ss [complete_def]
-   ++ METIS_TAC [sup_lub, inf_glb]);
+   >> METIS_TAC [sup_lub, inf_glb]);
 
 (* ------------------------------------------------------------------------- *)
 (* A calculator for rational posreals.                                       *)
@@ -1799,7 +1796,7 @@ val add_rat = store_thm
        else & (a * d + b * c) / & (b * d)``,
    RW_TAC std_ss [div_lzero, add_lzero, div_rzero, posreal_of_num_inj,
                   add_linfty, add_rzero, add_rinfty]
-   ++ RW_TAC std_ss [preal_div, posreal_of_num_def, REAL_POS, REAL_INJ,
+   >> RW_TAC std_ss [preal_div, posreal_of_num_def, REAL_POS, REAL_INJ,
                      MULT_EQ_0, ADD_EQ_0, REAL_LE_DIV, preal_add,
                      REAL_ADD_RAT, REAL_MUL, REAL_ADD]);
 
@@ -1812,9 +1809,9 @@ val add_ratl = store_thm
        else if b = 0 then infty
        else & (a + b * c) / & b``,
    REPEAT GEN_TAC
-   ++ MP_TAC (Q.SPEC `& c` div_rone)
-   ++ DISCH_THEN (fn th => CONV_TAC (LAND_CONV (ONCE_REWRITE_CONV [GSYM th])))
-   ++ RW_TAC std_ss
+   >> MP_TAC (Q.SPEC `& c` div_rone)
+   >> DISCH_THEN (fn th => CONV_TAC (LAND_CONV (ONCE_REWRITE_CONV [GSYM th])))
+   >> RW_TAC std_ss
       [add_rat, div_rone, mul_rone, div_lzero, div_rzero, posreal_of_num_inj,
        MULT_RIGHT_1]);
 
@@ -1840,15 +1837,15 @@ val sub_rat = store_thm
        else & (a * d - b * c) / & (b * d)``,
    RW_TAC std_ss [div_lzero, sub_lzero, div_rzero, posreal_of_num_inj,
                   sub_rzero, unint_def]
-   ++ RW_TAC std_ss [preal_div, posreal_of_num_def, REAL_POS, REAL_INJ,
+   >> RW_TAC std_ss [preal_div, posreal_of_num_def, REAL_POS, REAL_INJ,
                      sub_linfty, preal_not_infty, sub_rinfty,
                      MULT_EQ_0, ADD_EQ_0, REAL_LE_DIV, preal_sub,
                      REAL_SUB, REAL_SUB_RAT, REAL_MUL]
-   ++ RW_TAC std_ss
+   >> RW_TAC std_ss
       [preal_eq_zero, GSYM posreal_of_num_def, GSYM REAL_NEG_GE0,
        real_div, REAL_MUL_LNEG, REAL_NEGNEG]
-   ++ MATCH_MP_TAC REAL_LE_MUL
-   ++ RW_TAC std_ss [REAL_POS, REAL_LE_INV]);
+   >> MATCH_MP_TAC REAL_LE_MUL
+   >> RW_TAC std_ss [REAL_POS, REAL_LE_INV]);
 
 val sub_ratl = store_thm
   ("sub_ratl",
@@ -1859,10 +1856,10 @@ val sub_ratl = store_thm
        else if b = 0 then infty
        else & (a - b * c) / & b``,
    REPEAT GEN_TAC
-   ++ MP_TAC (Q.SPEC `& c` div_rone)
-   ++ DISCH_THEN (fn th => CONV_TAC (LAND_CONV (ONCE_REWRITE_CONV [GSYM th])))
-   ++ ONCE_REWRITE_TAC [sub_rat]
-   ++ RW_TAC std_ss
+   >> MP_TAC (Q.SPEC `& c` div_rone)
+   >> DISCH_THEN (fn th => CONV_TAC (LAND_CONV (ONCE_REWRITE_CONV [GSYM th])))
+   >> ONCE_REWRITE_TAC [sub_rat]
+   >> RW_TAC std_ss
       [div_rone, mul_rone, div_lzero, div_rzero, posreal_of_num_inj,
        MULT_RIGHT_1, sub_rzero, sub_lzero, sub_linfty,
        posreal_of_num_not_infty, preal_sub, preal_div, REAL_POS]);
@@ -1876,15 +1873,15 @@ val sub_ratr = store_thm
        else if b = 0 then 0
        else & (b * c - a) / & b``,
    REPEAT GEN_TAC
-   ++ MP_TAC (Q.SPEC `& c` div_rone)
-   ++ DISCH_THEN (fn th => CONV_TAC (LAND_CONV (ONCE_REWRITE_CONV [GSYM th])))
-   ++ ONCE_REWRITE_TAC [sub_rat]
-   ++ RW_TAC std_ss
+   >> MP_TAC (Q.SPEC `& c` div_rone)
+   >> DISCH_THEN (fn th => CONV_TAC (LAND_CONV (ONCE_REWRITE_CONV [GSYM th])))
+   >> ONCE_REWRITE_TAC [sub_rat]
+   >> RW_TAC std_ss
       [div_rone, mul_rone, div_lzero, div_rzero, posreal_of_num_inj,
        MULT_RIGHT_1, sub_rzero, sub_lzero, sub_linfty,
        posreal_of_num_not_infty, preal_sub, preal_div, REAL_POS,
        MULT_LEFT_1]
-   ++ METIS_TAC [MULT_COMM]);
+   >> METIS_TAC [MULT_COMM]);
 
 val sub_linfty_rat = store_thm
   ("sub_linfty_rat",
@@ -1918,13 +1915,13 @@ val mul_rat = store_thm
    ``!a b c d : num. (& a / & b) * (& c / & d) = & (a * c) / & (b * d)``,
    RW_TAC std_ss
    [preal_div_def, inv_mul, entire, posreal_of_num_inj, GSYM posreal_of_num_mul]
-   ++ Cases_on `a = 0`
-   ++ Cases_on `c = 0`
-   ++ RW_TAC std_ss
+   >> Cases_on `a = 0`
+   >> Cases_on `c = 0`
+   >> RW_TAC std_ss
       [mul_lzero, mul_rzero, mul_linfty, mul_rinfty, inv_zero,
        posreal_of_num_inj, inv_eq_zero, entire, posreal_of_num_not_infty]
-   ++ FULL_SIMP_TAC std_ss []
-   ++ METIS_TAC [mul_comm, mul_assoc]);
+   >> FULL_SIMP_TAC std_ss []
+   >> METIS_TAC [mul_comm, mul_assoc]);
 
 val mul_ratl = store_thm
   ("mul_ratl",
@@ -1970,15 +1967,15 @@ val div_rat = store_thm
        if c = 0 then if a = 0 then 0 else infty
        else & (a * d) / & (b * c)``,
    REPEAT GEN_TAC
-   ++ Cases_on `a = 0`
-   ++ Cases_on `b = 0`
-   ++ Cases_on `c = 0`
-   ++ Cases_on `d = 0`
-   ++ RW_TAC std_ss
+   >> Cases_on `a = 0`
+   >> Cases_on `b = 0`
+   >> Cases_on `c = 0`
+   >> Cases_on `d = 0`
+   >> RW_TAC std_ss
       [mul_lzero, mul_rzero, mul_linfty, mul_rinfty, inv_zero, inv_inv,
        posreal_of_num_inj, inv_eq_zero, entire, posreal_of_num_not_infty,
        preal_div_def, inv_mul, entire, GSYM posreal_of_num_mul, inv_eq_infty]
-   ++ METIS_TAC [mul_comm, mul_assoc]);
+   >> METIS_TAC [mul_comm, mul_assoc]);
 
 val div_ratl = store_thm
   ("div_ratl",
@@ -2021,70 +2018,71 @@ val div_linfty_rat = store_thm
 val le_rat = store_thm
   ("le_rat",
    ``!a b c d.
-       & a / & b <= & c / & d =
+       & a / & b <= & c / & d <=>
        if d = 0 then (a = 0) \/ ~(c = 0) else a * d <= b * c``,
    REPEAT GEN_TAC
-   ++ Cases_on `a = 0`
-   ++ Cases_on `b = 0`
-   ++ Cases_on `c = 0`
-   ++ Cases_on `d = 0`
-   ++ RW_TAC arith_ss
+   >> Cases_on `a = 0`
+   >> Cases_on `b = 0`
+   >> Cases_on `c = 0`
+   >> Cases_on `d = 0`
+   >> RW_TAC arith_ss
       [div_rzero, le_refl, zero_le, div_lzero, posreal_of_num_inj, le_infty,
        infty_le, posreal_of_num_not_infty, div_eq_infty, le_zero, div_eq_zero]
-   ++ RW_TAC std_ss [le_eq_sub_zero]
-   ++ ONCE_REWRITE_TAC [sub_rat]
-   ++ RW_TAC arith_ss
+   >> RW_TAC std_ss [le_eq_sub_zero]
+   >> ONCE_REWRITE_TAC [sub_rat]
+   >> RW_TAC arith_ss
       [div_eq_infty, posreal_of_num_inj, posreal_of_num_not_infty,
        div_eq_zero]);
 
 val le_ratl = store_thm
   ("le_ratl",
-   ``!c a b. & a / & b <= & c = a <= b * c``,
+   ``!c a b. & a / & b <= & c <=> a <= b * c``,
    METIS_TAC [le_rat, div_rone, MULT_RIGHT_1, ONE, SUC_NOT]);
 
 val le_ratr = store_thm
   ("le_ratr",
    ``!c a b.
-       & c <= & a / & b = if b = 0 then (c = 0) \/ ~(a = 0) else c * b <= a``,
+       & c <= & a / & b <=> if b = 0 then (c = 0) \/ ~(a = 0) else c * b <= a``,
    METIS_TAC [le_rat, div_rone, MULT_LEFT_1]);
 
 val eq_rat = store_thm
   ("eq_rat",
    ``!a b c d.
-       (& a / & b = & c / & d) =
+       (& a / & b = & c / & d) <=>
        if a = 0 then c = 0 else ~(c = 0) /\ (a * d = b * c)``,
    RW_TAC arith_ss [le_antisym_eq, le_rat]
-   ++ Cases_on `c = 0` >> RW_TAC arith_ss []
-   ++ METIS_TAC [LESS_EQUAL_ANTISYM, LESS_EQ_REFL, MULT_COMM]);
+   >> Cases_on `c = 0` >- RW_TAC arith_ss []
+   >> METIS_TAC [LESS_EQUAL_ANTISYM, LESS_EQ_REFL, MULT_COMM]);
 
 val eq_ratl = store_thm
   ("eq_ratl",
-   ``!a b c. (& a / & b = & c) = if a = 0 then c = 0 else a = b * c``,
+   ``!a b c. (& a / & b = & c) <=> if a = 0 then c = 0 else a = b * c``,
    REPEAT GEN_TAC
-   ++ MP_TAC (Q.SPEC `& c` div_rone)
-   ++ DISCH_THEN (fn th => CONV_TAC (LAND_CONV (ONCE_REWRITE_CONV [GSYM th])))
-   ++ RW_TAC std_ss [eq_rat, mul_rone]
-   ++ Cases_on `c = 0`
-   ++ RW_TAC std_ss [mul_rzero, MULT_0, MULT_RIGHT_1]);
+   >> MP_TAC (Q.SPEC `& c` div_rone)
+   >> DISCH_THEN (fn th => CONV_TAC (LAND_CONV (ONCE_REWRITE_CONV [GSYM th])))
+   >> RW_TAC std_ss [eq_rat, mul_rone]
+   >> Cases_on `c = 0`
+   >> RW_TAC std_ss [mul_rzero, MULT_0, MULT_RIGHT_1]);
 
 val rat_eq_infty = store_thm
   ("rat_eq_infty",
-   ``!a b. (& a / & b = infty) = ~(a = 0) /\ (b = 0)``,
+   ``!a b. (& a / & b = infty) <=> ~(a = 0) /\ (b = 0)``,
    RW_TAC std_ss [div_eq_infty, posreal_of_num_inj, posreal_of_num_not_infty]);
 
-val rat_cancel = store_thm
-  ("rat_cancel",
-   ``!a b c. (& a * & b) / (& a * & c) = if a = 0 then 0 else & b / & c``,
+Theorem rat_cancel:
+  !a b c. (& a * & b) / (& a * & c) = if a = 0 then 0 else & b / & c
+Proof
    (RW_TAC std_ss [preal_div_def, mul_lzero, inv_mul, entire,
                   posreal_of_num_inj]
-    ++ FULL_SIMP_TAC std_ss [DE_MORGAN_THM, inv_zero])
-   >> (Cases_on `& b = 0`
-       ++ RW_TAC std_ss [mul_assoc, mul_rinfty, mul_rzero, posreal_of_num_inj])
-   ++ MP_TAC (METIS_PROVE [mul_assoc, mul_comm]
+    >> FULL_SIMP_TAC std_ss [DE_MORGAN_THM, inv_zero])
+   >- (Cases_on `& b = 0`
+       >> RW_TAC std_ss [mul_assoc, mul_rinfty, mul_rzero, posreal_of_num_inj])
+   >> MP_TAC (METIS_PROVE [mul_assoc, mul_comm]
               ``!a b c d : posreal. (a * b) * (c * d) = (a * c) * (b * d)``)
-   ++ DISCH_THEN (fn th => ONCE_REWRITE_TAC [th])
-   ++ RW_TAC std_ss
-      [mul_rinv, posreal_of_num_not_infty, posreal_of_num_inj, mul_lone]);
+   >> DISCH_THEN (fn th => ONCE_REWRITE_TAC [th])
+   >> RW_TAC std_ss
+      [mul_rinv, posreal_of_num_not_infty, posreal_of_num_inj, mul_lone]
+QED
 
 val min_num = store_thm
   ("min_num",
@@ -2097,14 +2095,14 @@ val min_ratl = store_thm
        min (& a / & b) (& m) =
        if (a = 0) \/ a <= b * m then & a / & b else & m``,
    REPEAT STRIP_TAC
-   ++ Cases_on `a = 0` >> RW_TAC std_ss [div_lzero, min_lzero]
-   ++ RW_TAC std_ss [preal_min_def]
-   << [MATCH_MP_TAC le_antisym
-       ++ RW_TAC std_ss [le_ratr]
-       ++ PROVE_TAC [LESS_EQ_CASES, MULT_COMM, ZERO_LESS_EQ],
-       Suff `F` >> PROVE_TAC []
-       ++ Q.PAT_ASSUM `~(X <= Y)` MP_TAC
-       ++ RW_TAC std_ss [le_ratl]]);
+   >> Cases_on `a = 0` >- RW_TAC std_ss [div_lzero, min_lzero]
+   >> RW_TAC std_ss [preal_min_def]
+   >| [MATCH_MP_TAC le_antisym
+       >> RW_TAC std_ss [le_ratr]
+       >> PROVE_TAC [LESS_EQ_CASES, MULT_COMM, ZERO_LESS_EQ],
+       Suff `F` >- PROVE_TAC []
+       >> Q.PAT_X_ASSUM `~(X <= Y)` MP_TAC
+       >> RW_TAC std_ss [le_ratl]]);
 
 val min_ratr = store_thm
   ("min_ratr",
@@ -2120,11 +2118,11 @@ val min_rat = store_thm
        if (a = 0) \/ (~(c = 0) /\ d * a <= c * b) then & a / & b
        else & c / & d``,
    REPEAT STRIP_TAC
-   ++ Cases_on `a = 0` >> RW_TAC std_ss [div_lzero, min_lzero]
-   ++ Cases_on `c = 0` >> RW_TAC std_ss [div_lzero, min_rzero]
-   ++ RW_TAC std_ss [preal_min_def, eq_rat, le_rat]
-   ++ FULL_SIMP_TAC arith_ss []
-   ++ PROVE_TAC [MULT_COMM, LESS_EQ_CASES, LESS_EQUAL_ANTISYM]);
+   >> Cases_on `a = 0` >- RW_TAC std_ss [div_lzero, min_lzero]
+   >> Cases_on `c = 0` >- RW_TAC std_ss [div_lzero, min_rzero]
+   >> RW_TAC std_ss [preal_min_def, eq_rat, le_rat]
+   >> FULL_SIMP_TAC arith_ss []
+   >> PROVE_TAC [MULT_COMM, LESS_EQ_CASES, LESS_EQUAL_ANTISYM]);
 
 val max_num = store_thm
   ("max_num",
@@ -2137,14 +2135,14 @@ val max_ratl = store_thm
        max (& a / & b) (& m) =
        if (a = 0) \/ a <= b * m then & m else & a / & b``,
    REPEAT STRIP_TAC
-   ++ Cases_on `a = 0` >> RW_TAC std_ss [div_lzero, max_lzero]
-   ++ RW_TAC std_ss [preal_max_def]
-   << [MATCH_MP_TAC le_antisym
-       ++ RW_TAC std_ss [le_ratr]
-       ++ PROVE_TAC [LESS_EQ_CASES, MULT_COMM, ZERO_LESS_EQ],
-       Suff `F` >> PROVE_TAC []
-       ++ Q.PAT_ASSUM `~(X <= Y)` MP_TAC
-       ++ RW_TAC std_ss [le_ratl]]);
+   >> Cases_on `a = 0` >- RW_TAC std_ss [div_lzero, max_lzero]
+   >> RW_TAC std_ss [preal_max_def]
+   >| [MATCH_MP_TAC le_antisym
+       >> RW_TAC std_ss [le_ratr]
+       >> PROVE_TAC [LESS_EQ_CASES, MULT_COMM, ZERO_LESS_EQ],
+       Suff `F` >- PROVE_TAC []
+       >> Q.PAT_X_ASSUM `~(X <= Y)` MP_TAC
+       >> RW_TAC std_ss [le_ratl]]);
 
 val max_ratr = store_thm
   ("max_ratr",
@@ -2160,22 +2158,22 @@ val max_rat = store_thm
        if (a = 0) \/ (~(c = 0) /\ d * a <= c * b) then & c / & d
        else & a / & b``,
    REPEAT STRIP_TAC
-   ++ Cases_on `a = 0` >> RW_TAC std_ss [div_lzero, max_lzero]
-   ++ Cases_on `c = 0` >> RW_TAC std_ss [div_lzero, max_rzero]
-   ++ RW_TAC std_ss [preal_max_def, eq_rat, le_rat]
-   ++ FULL_SIMP_TAC arith_ss []
-   ++ PROVE_TAC [MULT_COMM, LESS_EQ_CASES, LESS_EQUAL_ANTISYM]);
+   >> Cases_on `a = 0` >- RW_TAC std_ss [div_lzero, max_lzero]
+   >> Cases_on `c = 0` >- RW_TAC std_ss [div_lzero, max_rzero]
+   >> RW_TAC std_ss [preal_max_def, eq_rat, le_rat]
+   >> FULL_SIMP_TAC arith_ss []
+   >> PROVE_TAC [MULT_COMM, LESS_EQ_CASES, LESS_EQUAL_ANTISYM]);
 
 val bound1_num = store_thm
   ("bound1_num",
    ``!m. bound1 (& m) = if m = 0 then 0 else 1``,
    RW_TAC std_ss [bound1_min, min_num, posreal_of_num_inj]
-   ++ DECIDE_TAC);
+   >> DECIDE_TAC);
 
 val bound1_rat = store_thm
   ("bound1_rat",
    ``!a b. bound1 (& a / & b) = if a <= b then & a / & b else 1``,
    RW_TAC std_ss [bound1_min, min_ratl]
-   ++ FULL_SIMP_TAC arith_ss []);
+   >> FULL_SIMP_TAC arith_ss []);
 
 val _ = export_theory();
